# Copyright 2016 ITEA 12004 SEAS Project.
# 
# Licensed under the Apache License, Version 2.0 (the "License");
# you may not use this file except in compliance with the License.
# You may obtain a copy of the License at
# 
#      http://www.apache.org/licenses/LICENSE-2.0
# 
# Unless required by applicable law or agreed to in writing,
# distributed under the License is distributed on an "AS IS" BASIS,
# WITHOUT WARRANTIES OR CONDITIONS OF ANY KIND, either express or implied.
# See the License for the specific language governing permissions and
# limitations under the License.

@prefix rdf: <http://www.w3.org/1999/02/22-rdf-syntax-ns#> . #Resource data framework
@prefix owl: <http://www.w3.org/2002/07/owl#> .              #Owl ontology language
@prefix rdfs: <http://www.w3.org/2000/01/rdf-schema#> .      #RDF schema 
@prefix xsd: <http://www.w3.org/2001/XMLSchema#> .           #XML standard datatypes
@prefix dc: <http://purl.org/dc/terms/> .     #Dublin Core Metadata Initiative terms
@prefix vann: <http://purl.org/vocab/vann/> .  #A vocabulary for annotating vocabulary descriptions
@prefix voaf: <http://purl.org/vocommons/voaf#> . #A vocabulary of a friend, for describing relations between linked vocabularies
@prefix vs: <http://www.w3.org/2003/06/sw-vocab-status/ns#> . #Semantic web vocabulary status ontology
@prefix cc: <http://creativecommons.org/ns#>.
@prefix foaf: <http://xmlns.com/foaf/0.1/>.

@prefix seas: <https://w3id.org/seas/>.
@base <https://w3id.org/seas/>.

#SEAS architecture related concepts
seas:ArchitectureOntology rdf:type voaf:Vocabulary , owl:Ontology ;
  dc:title "SEAS-ArchitectureOntology ontology"@en ;
  dc:description "The Seas Architecture Ontology for the ITEA SEAS (Smart Energy Aware Systems) project."@en ;
  dc:issued "2016-01-26"^^xsd:date ;
  dc:modified "2016-06-25"^^xsd:date ;
  dc:author <http://www.maxime-lefrancois.info/me#> ;
  dc:contributor [a foaf:Person ; foaf:name "Guillaume Habault" ] ;
  dc:contributor [a foaf:Person ; foaf:name "Jani Hursti" ] ;
  cc:license <https://creativecommons.org/licenses/by/4.0> ;
  vann:preferredNamespacePrefix "seas" ;
  vann:preferredNamespaceUri <https://w3id.org/seas/> ;  
  # owl:imports <https://w3id.org/seas/SystemOntology> ;
  owl:versionIRI <https://w3id.org/seas/ArchitectureOntology/2.0> ;
  owl:versionInfo "v2.0" .

## electric power system

seas:Entity a owl:Class ;
  rdfs:label "SEAS Entity"@en ;
  rdfs:comment """The class SEAS entity represents the abstract class of communicating nodes."""@en ;
  rdfs:subClassOf seas:System ;
  vs:term_status "testing" ;
  rdfs:isDefinedBy seas:ArchitectureOntology .

seas:CoreEntity a owl:Class ;
  rdfs:label "SEAS Core Entity"@en ;
  rdfs:comment """SEAS core entities are SEAS nodes that belong to the SEAS core domain. 
  The SEAS core domain is where all SEAS core entities, group managers, and SEAS core services can be interconnected.
  Interconnections within the SEAS core domain all rely on the Internet Protocol. 

  SEAS core entities can be connected to other SEAS core entities in a peer-to-peer basis, and exchange information.
  SEAS core entities can be connected to SEAS field entities, provided that they have sufficient access right."""@en ;
  rdfs:subClassOf seas:Entity ;
  vs:term_status "testing" ;
  rdfs:isDefinedBy seas:ArchitectureOntology .

  seas:RegistrationEntity a owl:Class ;
    rdfs:label "Registration Entity"@en ;
    rdfs:comment """The class of entities that provide the SEAS core registration services for SEAS core entities.

    A SEAS registration service is an API that enables SEAS core services to register themselves along with their capabilities for others to find them.

    The complete specification of the SEAS core registration services is available in SEAS Deliverable X.X."""@en ;
    rdfs:subClassOf seas:CoreEntity ;
    vs:term_status "testing" ;
    rdfs:isDefinedBy seas:ArchitectureOntology .

  seas:TransactionEntity a owl:Class ;
    rdfs:label "Transaction Entity"@en ;
    rdfs:comment """The class of entities that provide the SEAS core transaction services for SEAS core entities.

    A SEAS core transaction service is an API that connects SEAS core entities to banks and payment systems, and acts as a trusted notary to enable compensation for participation in SEAS field entities management.

    The complete specification of the SEAS core transaction services is available in SEAS Deliverable X.X."""@en ;
    rdfs:subClassOf seas:CoreEntity ;
    vs:term_status "testing" ;
    rdfs:isDefinedBy seas:ArchitectureOntology .

  seas:OntologyEntity a owl:Class ;
    rdfs:label "Ontology Entity" ;
    rdfs:comment """The class of entities that provide the SEAS core ontology services for SEAS core entities.

    A SEAS core ontology service is an API that exposes media types descriptions, notably information about:
     - how to validate a document with a specific media type;
     - how to lift a document with a specific media type to RDF;
     - how to validate a RDF Graph; 
     - how to lower a RDF Graph to a document with a specific media type.

    The complete specification of the SEAS core ontology services is available in SEAS Deliverable X.X."""@en ;
    rdfs:subClassOf seas:CoreEntity ;
    vs:term_status "testing" ;
    rdfs:isDefinedBy seas:ArchitectureOntology .

  seas:SecurityEntity a owl:Class ; 
    rdfs:label "Security Entity"@en ;
    rdfs:comment """The class of entities that provide the SEAS core security services for SEAS core entities.

    A SEAS core security service is an API that enable:
     - SEAS core entities to communicate their access control preferences;
     - SEAS core entities to control the access rights of other SEAS core entities for some type information.

    The complete specification of the SEAS core security services is available in SEAS Deliverable X.X."""@en ;
    rdfs:subClassOf seas:CoreEntity ;
    vs:term_status "testing" ;
    rdfs:isDefinedBy seas:ArchitectureOntology .

  seas:EndUser a owl:Class ; 
    rdfs:label "End User"@en ;
    rdfs:comment """The class of end user entities, that own SEAS field entities."""@en ;
    rdfs:subClassOf seas:CoreEntity ;
    vs:term_status "testing" ;
    rdfs:isDefinedBy seas:ArchitectureOntology .

# field entity

seas:FieldEntity a owl:Class ;
  rdfs:label "SEAS Field Entity"@en ;
  rdfs:comment """SEAS field entities are SEAS nodes that belong to the SEAS field domain.
  The SEAS field domain is the the link with the physical world.

  SEAS field entities can be connected to other SEAS field entities in a client-server basis.

  SEAS field entities can belong to one or several SEAS groups.
  Every SEAS group is managed by exactly one group manager.
  Field entities participate in the management of the group."""@en ;
  rdfs:subClassOf seas:Entity ;
  vs:term_status "testing" ;
  rdfs:isDefinedBy seas:ArchitectureOntology .

  seas:GroupManager a owl:Class ;
    rdfs:label "SEAS Group Manager"@en ;
    rdfs:comment """SEAS group managers are both field and core entities. 
    They manage exactly one group."""@en ;
    rdfs:subClassOf seas:CoreEntity , seas:FieldEntity ;
    owl:equivalentClass [ owl:intersectionOf ( seas:CoreEntity seas:FieldEntity ) ] ;
    vs:term_status "testing" ;
    rdfs:isDefinedBy seas:ArchitectureOntology .

# connections

seas:exchangesInformationWith a owl:ObjectProperty , owl:SymmetricProperty ;
  rdfs:label "exchanges information with"@en ;
  rdfs:comment """Links a SEAS core entity to another SEAS core entity it exchanges information with. 

  This property can be qualified using class seas:CoreEntityConnection, which connects (at least) the two core entities.
  For example, for information to flow between a system operator and a market operator, then they must share a core entity connection:

  <system_operator> a seas:CoreEntity .
  <market_operator> a seas:CoreEntity .
  <system_operator> seas:exchangesInformationWith <market_operator> . 

  If there is a core entity connection between several core entities, then one may infer these core entities can exchange information."""@en ;
  rdfs:subPropertyOf seas:connectedTo ;
  rdfs:domain seas:CoreEntity ;
  rdfs:range seas:CoreEntity ;
  vs:term_status "testing" ;
  rdfs:isDefinedBy seas:ArchitectureOntology .

seas:directlyAccesses a owl:ObjectProperty ;
  rdfs:label "directly accesses"@en ;
  rdfs:comment """Links a SEAS core entity to a SEAS field entity it has direct access to. 

  This property can be qualified using class seas:DirectAccessConnection, which connects the core entity and the field entity.
  For example, for a flexibility operator to directly access a solar panel, then it must have a direct access connection to it:

  <flexibility_operator> a seas:CoreEntity .
  <solar_panel> a seas:FieldEntity .
  <flexibility_operator> seas:accessesDirectly <solar_panel> . 

  If there is a direct access connection between a core entity and a field entity, then one may infer the core entity can directly access the field entity."""@en ;
  rdfs:subPropertyOf seas:connectedTo ;
  rdfs:domain seas:CoreEntity ;
  rdfs:range seas:FieldEntity ;
  owl:inverseOf seas:directlyAccessedBy ;
  vs:term_status "testing" ;
  rdfs:isDefinedBy seas:ArchitectureOntology .

seas:directlyAccessedBy a owl:ObjectProperty ;
  rdfs:label "directly accesses by"@en ;
  rdfs:comment """Links a SEAS field entity to a core entity that directly accesses it. 

  This property can be qualified using class seas:DirectAccessConnection, which connects the core entity and the field entity.
  For example, for a flexibility operator to directly access a solar panel, then it must have a direct access connection to it:

  <flexibility_operator> a seas:CoreEntity .
  <solar_panel> a seas:FieldEntity .
  <solar_panel> seas:accessesDirectly <flexibility_operator> . 

  If there is a direct access connection between a core entity and a field entity, then one may infer the core entity can directly access the field entity."""@en ;
  rdfs:subPropertyOf seas:connectedTo ;
  rdfs:domain seas:FieldEntity ;
  rdfs:range seas:CoreEntity ;
  owl:inverseOf seas:directlyAccesses ;
  vs:term_status "testing" ;
  rdfs:isDefinedBy seas:ArchitectureOntology .


seas:directlyManages a owl:ObjectProperty , owl:InverseFunctionalProperty ;
  rdfs:label "directly manages"@en ;
  rdfs:comment """Links a SEAS group manager to a SEAS field entity it directly manages. 

  This property can be qualified using class seas:DirectManagementConnection, which connects the group manager and the field entities it directly manages.
  For example, for a home management system to directly manage a smart fridge, then it must have a management connection to it:

  <home_management_system> a seas:GroupManager .
  <smart_fridge> a seas:FieldEntity .
  <home_management_system> seas:directlyManages <smart_fridge> . 

  If there is a direct management connection between a group manager and a field entity, then one may infer the group manager directly manages the field entity."""@en ;
  rdfs:subPropertyOf seas:connectedTo ;
  rdfs:domain seas:GroupManager ;
  rdfs:range seas:FieldEntity ;
  owl:inverseOf seas:directlyManagedBy ;
  vs:term_status "testing" ;
  rdfs:isDefinedBy seas:ArchitectureOntology .

seas:directlyManagedBy a owl:ObjectProperty , owl:FunctionalProperty ;
  rdfs:label "directly managed by"@en ;
  rdfs:comment """Links a SEAS field entity to the group manager that directly manages it. 

  This property can be qualified using class seas:DirectManagementConnection, which connects the group manager and the field entities it directly manages.
  For example, for a home management system to directly manage a smart fridge, then it must have a management connection to it:

  <home_management_system> a seas:GroupManager .
  <smart_fridge> a seas:FieldEntity .
  <home_management_system> seas:directlyManages <smart_fridge> . 

  If there is a direct management connection between a group manager and a field entity, then one may infer the group manager directly manage the field entity."""@en ;
  rdfs:subPropertyOf seas:connectedTo ;
  rdfs:domain seas:FieldEntity ;
  rdfs:range seas:GroupManager ;
  owl:inverseOf seas:directlyManages ;
  vs:term_status "testing" ;
  rdfs:isDefinedBy seas:ArchitectureOntology .


## electrical connection

seas:EntityConnection a owl:Class ;
  rdfs:label "Entity Connection"@en ;
  rdfs:comment """The class of entity connections between SEAS entities."""@en ;
  rdfs:subClassOf seas:Connection ;
  rdfs:subClassOf [ owl:onProperty seas:connectsSystem ; owl:allValuesFrom  seas:Entity ] ;
  rdfs:subClassOf [ owl:onProperty seas:connectsSystemAt ; owl:allValuesFrom  seas:EntityAccessPoint ] ;
  vs:term_status "testing" ;
  rdfs:isDefinedBy seas:ArchitectureOntology .

  seas:CoreEntityConnection a owl:Class ;
    rdfs:label "Core Entity Connection"@en ;
    rdfs:comment """The class of SEAS core entity connections between SEAS core entities.
    SEAS core entity connections describe potential information flows between the SEAS core entities it connects.
    For example, the following RDF graph states that a SEAS core entity connection connects a home management system with an aggregator and the transaction server:

    <connection> a seas:ElectricalConnection ;
      seas:connectsSystem <home_management_system> , <aggregator> , <transaction_server> .

    Only SEAS core entities are connected through a SEAS core entity connection.
    A connection between SEAS core entities is not necessarily a SEAS core entity connection."""@en ;
    rdfs:subClassOf seas:EntityConnection ;
    rdfs:subClassOf [ owl:onProperty seas:connectsSystem ; owl:allValuesFrom  seas:CoreEntity ] ;
    vs:term_status "testing" ;
    rdfs:isDefinedBy seas:ArchitectureOntology .

  seas:DirectAccessConnection a owl:Class ;
    rdfs:label "Direct Access Connection"@en ;
    rdfs:comment """The class of SEAS direct access connections between a SEAS core entity and one or more SEAS field entities it directly accesses.
    Direct access connections describe potential control of the SEAS core entity to the SEAS field entities.
    For example, the following RDF graph states that a SEAS direct access connection connects a distribution system operator with a solar panel:

    <connection> a seas:DirectAccessConnection ;
      seas:connectsSystem <distribution_system_operator> , <solar_panel> .

    Only SEAS entities are connected through a direct access connection.
    A connection between SEAS entities is not necessarily a direct access connection."""@en ;
    rdfs:subClassOf seas:EntityConnection ;
    owl:disjointWith seas:CoreEntityConnection ;
    vs:term_status "testing" ;
    rdfs:isDefinedBy seas:ArchitectureOntology .

  seas:DirectManagementConnection a owl:Class ;
    rdfs:label "Direct Management Connection"@en ;
    rdfs:comment """The class of SEAS direct management connections between a SEAS group manager entity and each of the entities it directly manages (i.e., the group).
    Direct management connections describe the management of the SEAS field entities by the SEAS group manager.
    For example, the following RDF graph states that a home management system manages a group of field entities composed of a solar panel and a battery:

    <connection> a seas:DirectManagementConnection ;
      seas:connectsSystem <home_management_system> , <solar_panel> , <battery> .

    Only SEAS entities and SEAS field entities are connected through a direct management connection.
    A connection between SEAS entities is not necessarily a direct management connection."""@en ;
    rdfs:subClassOf seas:EntityConnection ;
    owl:disjointWith seas:CoreEntityConnection , seas:DirectManagementConnection ;
    vs:term_status "testing" ;
    rdfs:isDefinedBy seas:ArchitectureOntology .


## entity access point

seas:EntityAccessPoint a owl:Class ;
  rdfs:label "Entity Access Point"@en ;
  rdfs:comment """The class of access points of SEAS entities, at which they may access or be accessed by other entities.
  For example, a solar panel may have an access point where smart grid management systems can access the latest information about its electricity production.

  An entity access point describes the APIs that one may use to access the system.
  An entity access point only belongs to one entity, and connects it through entity connections.
  A connection point of an entity is not necessarily an entity access point."""@en ;
  rdfs:subClassOf seas:ConnectionPoint ;
  rdfs:subClassOf [ owl:onProperty seas:connectionPointOf ; owl:allValuesFrom  seas:Entity ] ;
  rdfs:subClassOf [ owl:onProperty seas:connectsSystemThrough ; owl:allValuesFrom  seas:EntityConnection ] ;
  vs:term_status "testing" ;
  rdfs:isDefinedBy seas:ArchitectureOntology .
