@prefix : <https://w3id.org/seas/BuildingOntology#> .
@prefix vs: <http://www.w3.org/2003/06/sw-vocab-status/ns#> .
@prefix ifc: <http://www.buildingsmart-tech.org/ifcOWL/IFC2X3_TC1#> .
@prefix owl: <http://www.w3.org/2002/07/owl#> .
@prefix rdf: <http://www.w3.org/1999/02/22-rdf-syntax-ns#> .
@prefix xml: <http://www.w3.org/XML/1998/namespace> .
@prefix xsd: <http://www.w3.org/2001/XMLSchema#> .
@prefix foaf: <http://xmlns.com/foaf/0.1/> .
@prefix rdfs: <http://www.w3.org/2000/01/rdf-schema#> .
@prefix seas: <https://w3id.org/seas/> .
@prefix vann: <http://purl.org/vocab/vann/> .
@prefix voaf: <http://purl.org/vocommons/voaf#> .
@prefix gbxml: <http://www.gbxml.org/schema#> .
@prefix saref: <http://ontology.tno.nl/saref#> .
@prefix dcterms: <http://purl.org/dc/terms/> .
@prefix fiemser: <http://sites.google.com/site/smartappliancesproject/ontologies/fiemser#> .
@base <https://w3id.org/seas/BuildingOntology> .

<https://w3id.org/seas/BuildingOntology> rdf:type owl:Ontology ;
                                          owl:versionIRI seas:BuildingOntology-1.0 ;
                                          owl:imports seas:ZoneOntology ;
                                          dcterms:description """The SEAS Building ontology describes a taxonomy of buildings, building spaces, and rooms.

Some categorizations are based on the energy efficiency related to their insulation etc., although the actual values for classes depend the country specific regulations and geographical locations.

Other categorizations are based on occupancy and activities. There is no single accepted categorization available. This taxonomy uses some types selected from:

- International building occupancy based categories (USA)
- The Classification of Types of Constructions (EU)
- Finnish building categorization VTJ2000 (Finland)
- Wikipedia category page for Rooms: https://en.wikipedia.org/wiki/Category:Rooms

This ontology should limit the overlap with the following existing specialized ontologies:

- [FIEMSER ontology](http://sites.google.com/site/smartappliancesproject/ontologies/fiemser#).
- [gbXML ontology](http://www.gbxml.org/).
- [ifcOWL ontology](http://www.buildingsmart-tech.org/ifcOWL/IFC4), which is a OWL version of the Building Information Model standard.
- the potential ontology that might be developed in the context of the [Linked Building Data community group](https://www.w3.org/community/lbd/), or its successor Working Group.
"""@en ;
                                          vann:preferredNamespacePrefix "seas" ;
                                          owl:versionInfo "v1.0" ;
                                          dcterms:contributor [ foaf:name "Francisco Silva" ;
                                                                rdf:type foaf:Person
                                                              ] ,
                                                              [ foaf:name "Gabriel Santos" ;
                                                                rdf:type foaf:Person
                                                              ] ,
                                                              [ foaf:name "Brigida Teixeira" ;
                                                                rdf:type foaf:Person
                                                              ] ;
                                          dcterms:title "The SEAS Building Ontology"@en ;
                                          dcterms:issued "2016-01-26"^^xsd:date ;
                                          owl:priorVersion seas:BuildingOntology-0.9 ;
                                          dcterms:creator <http://www.vtt.fi/JarmoKalaoja> ;
                                          vann:preferredNamespaceUri seas: ;
                                          dcterms:contributor "Georg Ferdinand Schneider"^^xsd:string ;
                                          dcterms:modified "2016-09-26"^^xsd:date ;
                                          dcterms:creator <http://www.maxime-lefrancois.info/me#> ;
                                          dcterms:license <https://www.apache.org/licenses/LICENSE-2.0> .

#################################################################
#    Annotation properties
#################################################################

###  http://purl.org/dc/terms/contributor
dcterms:contributor rdf:type owl:AnnotationProperty .


###  http://purl.org/dc/terms/creator
dcterms:creator rdf:type owl:AnnotationProperty .


###  http://purl.org/dc/terms/description
dcterms:description rdf:type owl:AnnotationProperty .


###  http://purl.org/dc/terms/issued
dcterms:issued rdf:type owl:AnnotationProperty .


###  http://purl.org/dc/terms/license
dcterms:license rdf:type owl:AnnotationProperty .


###  http://purl.org/dc/terms/modified
dcterms:modified rdf:type owl:AnnotationProperty .


###  http://purl.org/dc/terms/title
dcterms:title rdf:type owl:AnnotationProperty .


###  http://purl.org/vocab/vann/preferredNamespacePrefix
vann:preferredNamespacePrefix rdf:type owl:AnnotationProperty .


###  http://purl.org/vocab/vann/preferredNamespaceUri
vann:preferredNamespaceUri rdf:type owl:AnnotationProperty .


###  http://www.w3.org/2003/06/sw-vocab-status/ns#term_status
vs:term_status rdf:type owl:AnnotationProperty .


#################################################################
#    Data properties
#################################################################

###  http://xmlns.com/foaf/0.1/name
foaf:name rdf:type owl:DatatypeProperty .


#################################################################
#    Classes
#################################################################

###  http://purl.org/vocommons/voaf#Vocabulary
voaf:Vocabulary rdf:type owl:Class .


###  http://xmlns.com/foaf/0.1/Person
foaf:Person rdf:type owl:Class .


###  https://w3id.org/seas/AssemblyBuilding
seas:AssemblyBuilding rdf:type owl:Class ;
                      rdfs:subClassOf seas:NonResidentalBuilding ;
                      rdfs:comment "places used for people gathering for entertainment, worship, and eating or drinking. Examples: churches, restaurants."@en ;
                      rdfs:isDefinedBy <https://w3id.org/seas/BuildingOntology> ;
                      rdfs:label "AssemblyBuilding"@en ,
                                 "Kokoontumisrakennus"@fi ;
                      vs:term_status "testing" .


###  https://w3id.org/seas/Attic
seas:Attic rdf:type owl:Class ;
           rdfs:subClassOf seas:Room ;
           rdfs:comment "the part of a building, especially of a house, directly under a roof; garret."@en ;
           rdfs:isDefinedBy <https://w3id.org/seas/BuildingOntology> ;
           rdfs:label "Attic"@en ;
           vs:term_status "testing" .


###  https://w3id.org/seas/Balcony
seas:Balcony rdf:type owl:Class ;
             rdfs:subClassOf seas:BuildingSpace ;
             rdfs:comment "An accessible structure extending from a building, especially outside a window."@en ;
             rdfs:isDefinedBy <https://w3id.org/seas/BuildingOntology> ;
             rdfs:label "Balcony"@en ;
             vs:term_status "testing" .


###  https://w3id.org/seas/Basement
seas:Basement rdf:type owl:Class ;
              rdfs:subClassOf seas:BuildingStorey ;
              rdfs:comment "A story of a building, partly or wholly underground."@en ;
              rdfs:isDefinedBy <https://w3id.org/seas/BuildingOntology> ;
              rdfs:label "Basement"@en ;
              vs:term_status "testing" .


###  https://w3id.org/seas/Bathroom
seas:Bathroom rdf:type owl:Class ;
              rdfs:subClassOf seas:Room ;
              rdfs:comment "Bathroom is mainly used for bathing &amp; washing up related activities."@en ;
              rdfs:isDefinedBy <https://w3id.org/seas/BuildingOntology> ;
              rdfs:label "Bathroom"@en ;
              vs:term_status "testing" .


###  https://w3id.org/seas/Bedroom
seas:Bedroom rdf:type owl:Class ;
             rdfs:subClassOf seas:Room ;
             rdfs:comment "Bedroom is used mainly for sleeping."@en ;
             rdfs:isDefinedBy <https://w3id.org/seas/BuildingOntology> ;
             rdfs:label "Bedroom"@en ;
             vs:term_status "testing" .


###  https://w3id.org/seas/Building
seas:Building rdf:type owl:Class ;
              rdfs:subClassOf seas:BuildingSpace ,
                              seas:Construction ,
                              seas:Zone ;
              rdfs:comment "Buildings are roofed constructions which can be used separately, have been built for permanent purposes, can be entered by persons and are suitable or intended for protecting persons, animals or objects."@en ;
              rdfs:isDefinedBy <https://w3id.org/seas/BuildingOntology> ;
              rdfs:label "Building"@en ;
              vs:term_status "testing" .


###  https://w3id.org/seas/BuildingSpace
seas:BuildingSpace rdf:type owl:Class ;
                   rdfs:subClassOf seas:Zone ;
                   rdfs:comment "A Space is a 3D volume bounded by surfaces. According to the FIEMSER definition, a building space in SAREF defines the physical spaces of the building."@en ;
                   rdfs:isDefinedBy <https://w3id.org/seas/BuildingOntology> ;
                   rdfs:label "BuildingSpace"@en ;
                   vs:term_status "testing" .


###  https://w3id.org/seas/BuildingSpaceConnection
seas:BuildingSpaceConnection rdf:type owl:Class ;
                             rdfs:subClassOf seas:ZoneConnection ,
                                             [ rdf:type owl:Restriction ;
                                               owl:onProperty seas:connectsSystem ;
                                               owl:allValuesFrom seas:BuildingSpace
                                             ] ,
                                             [ rdf:type owl:Restriction ;
                                               owl:onProperty seas:connectsSystemAt ;
                                               owl:allValuesFrom seas:BuildingSpaceFrontier
                                             ] ;
                             rdfs:comment "Connection between two building spaces, where they may potentially exchange heat, humidity, agents."@en ;
                             rdfs:isDefinedBy <https://w3id.org/seas/BuildingOntology> ;
                             rdfs:label "Building Space Connection"@en ;
                             vs:term_status "testing" .


###  https://w3id.org/seas/BuildingSpaceFrontier
seas:BuildingSpaceFrontier rdf:type owl:Class ;
                           rdfs:subClassOf seas:ZoneFrontier ,
                                           [ rdf:type owl:Restriction ;
                                             owl:onProperty seas:connectionPointOf ;
                                             owl:allValuesFrom seas:BuildingSpace
                                           ] ,
                                           [ rdf:type owl:Restriction ;
                                             owl:onProperty seas:connectsSystemThrough ;
                                             owl:allValuesFrom seas:BuildingSpaceConnection
                                           ] ;
                           rdfs:comment "Surface that marks the frontier of a building space, and represents the connection point to other building spaces."@en ;
                           rdfs:isDefinedBy <https://w3id.org/seas/BuildingOntology> ;
                           rdfs:label "Building Space Frontier"@en ;
                           vs:term_status "testing" .


###  https://w3id.org/seas/BuildingSpatialStructure
seas:BuildingSpatialStructure rdf:type owl:Class ;
                              rdfs:subClassOf seas:BuildingSpace ;
                              rdfs:comment "A man made structure with spatial properties."@en ;
                              rdfs:isDefinedBy <https://w3id.org/seas/BuildingOntology> ;
                              rdfs:label "BuildingSpatialStructure"@en ;
                              vs:term_status "testing" .


###  https://w3id.org/seas/BuildingStorey
seas:BuildingStorey rdf:type owl:Class ;
                    rdfs:subClassOf seas:BuildingSpatialStructure ;
                    rdfs:comment "The storey represents a (nearly) horizontal aggregation of spaces that are vertically bound."@en ;
                    rdfs:isDefinedBy <https://w3id.org/seas/BuildingOntology> ;
                    rdfs:label "BuildingStorey"@en ;
                    vs:term_status "testing" .


###  https://w3id.org/seas/Ceiling
seas:Ceiling rdf:type owl:Class ;
             rdfs:subClassOf seas:BuildingSpaceFrontier ;
             rdfs:comment "Ceiling is a downwards tilted horizontal surface."@en ;
             rdfs:isDefinedBy <https://w3id.org/seas/BuildingOntology> ;
             rdfs:label "Ceiling"@en ;
             vs:term_status "testing" .


###  https://w3id.org/seas/CivilEngineeringWork
seas:CivilEngineeringWork rdf:type owl:Class ;
                          rdfs:subClassOf seas:Construction ;
                          rdfs:comment "Civil engineering works are all constructions not classified under buildings : railways, roads, bridges, highways, airport runways, dams etc."@en ;
                          rdfs:isDefinedBy <https://w3id.org/seas/BuildingOntology> ;
                          rdfs:label "CivilEngnineeringWork"@en ;
                          vs:term_status "testing" .


###  https://w3id.org/seas/ClosedBuildingSpaceConnection
seas:ClosedBuildingSpaceConnection rdf:type owl:Class ;
                                   rdfs:subClassOf seas:BuildingSpaceConnection ;
                                   owl:disjointWith seas:OpenBuildingSpaceConnection ,
                                                    seas:OpennableBuildingSpaceConnection ;
                                   rdfs:comment """A closed building space connection is a closed connection between two building spaces. 

  This separation may for instance be a wall, i.e., a (tilted more than 60 percent) vertical surface. 

  Instances of `seas:ClosedBuildingSpaceConnection` may be typed by classes from specialized building ontologies."""@en ;
                                   rdfs:isDefinedBy <https://w3id.org/seas/BuildingOntology> ;
                                   rdfs:label "Closed Building Space Connection"@en ;
                                   vs:term_status "testing" .


###  https://w3id.org/seas/Construction
seas:Construction rdf:type owl:Class ;
                  rdfs:subClassOf seas:Zone ;
                  rdfs:comment "Constructions are structures connected with the ground which are made of construction materials and components and/or for which construction work is carried out."@en ;
                  rdfs:isDefinedBy <https://w3id.org/seas/BuildingOntology> ;
                  rdfs:label "Construction"@en ;
                  vs:term_status "testing" .


###  https://w3id.org/seas/Corridor
seas:Corridor rdf:type owl:Class ;
              rdfs:subClassOf seas:Lobby ;
              rdfs:comment "A gallery or passage connecting parts of a building; hallway."@en ;
              rdfs:isDefinedBy <https://w3id.org/seas/BuildingOntology> ;
              rdfs:label "Corridor"@en ;
              vs:term_status "testing" .


###  https://w3id.org/seas/DiningRoom
seas:DiningRoom rdf:type owl:Class ;
                rdfs:subClassOf seas:Room ;
                rdfs:comment "A room in which meals are eaten, as in a home or hotel, especially the room in which the major or more formal meals are eaten."@en ;
                rdfs:isDefinedBy <https://w3id.org/seas/BuildingOntology> ;
                rdfs:label "Dining Room"@en ;
                vs:term_status "testing" .


###  https://w3id.org/seas/Door
seas:Door rdf:type owl:Class ;
          rdfs:subClassOf seas:BuildingSpaceConnection ;
          rdfs:comment "the large flat piece of wood, glass etc that you move when you go into or out of a building, room, vehicle etc, or when you open a cupboard (Longman Dictionary of Contemporary English Online)"@en ;
          rdfs:isDefinedBy <https://w3id.org/seas/BuildingOntology> ;
          rdfs:label "Door"@en ;
          vs:term_status "testing" .


###  https://w3id.org/seas/EducationalBuilding
seas:EducationalBuilding rdf:type owl:Class ;
                         rdfs:subClassOf seas:NonResidentalBuilding ;
                         rdfs:comment "Schools and day care centers."@en ;
                         rdfs:isDefinedBy <https://w3id.org/seas/BuildingOntology> ;
                         rdfs:label "EducationalBuilding"@en ,
                                    "Opetusrakennus"@fi ;
                         vs:term_status "testing" .


###  https://w3id.org/seas/Elevator
seas:Elevator rdf:type owl:Class ;
              rdfs:subClassOf seas:BuildingSpace ;
              rdfs:comment "Elevator is used to transport people between different floors."@en ;
              rdfs:isDefinedBy <https://w3id.org/seas/BuildingOntology> ;
              rdfs:label "Elevator"@en ;
              vs:term_status "testing" .


###  https://w3id.org/seas/Floor
seas:Floor rdf:type owl:Class ;
           rdfs:subClassOf seas:BuildingSpaceFrontier ;
           rdfs:comment "A floor is a upwards tilted horzontal surface, could be divided to interior, exposed (outside) or raised floor."@en ;
           rdfs:isDefinedBy <https://w3id.org/seas/BuildingOntology> ;
           rdfs:label "Floor"@en ;
           vs:term_status "testing" .


###  https://w3id.org/seas/Garage
seas:Garage rdf:type owl:Class ;
            rdfs:subClassOf seas:Room ;
            rdfs:comment "Room for garage."@en ;
            rdfs:isDefinedBy <https://w3id.org/seas/BuildingOntology> ;
            rdfs:label "Garage"@en ;
            vs:term_status "testing" .


###  https://w3id.org/seas/Greenhouse
seas:Greenhouse rdf:type owl:Class ;
                rdfs:subClassOf seas:BuildingSpace ;
                rdfs:comment "A building, room, or zone, usually chiefly of glass, in which the temperature is maintained within a desired range, used for cultivating tender plants or growing plants out of season."@en ;
                rdfs:isDefinedBy <https://w3id.org/seas/BuildingOntology> ;
                rdfs:label "Greenhouse"@en ;
                vs:term_status "testing" .


###  https://w3id.org/seas/Hall
seas:Hall rdf:type owl:Class ;
          rdfs:subClassOf seas:Lobby ;
          rdfs:comment "A large entrance room of a house or building."@en ;
          rdfs:isDefinedBy <https://w3id.org/seas/BuildingOntology> ;
          rdfs:label "Hall"@en ;
          vs:term_status "testing" .


###  https://w3id.org/seas/HolidayBuilding
seas:HolidayBuilding rdf:type owl:Class ;
                     rdfs:subClassOf seas:ResidentalBuilding ;
                     rdfs:comment "A secondary residential building used only occasionally during vacations such as a summerhouse or cottage. "@en ;
                     rdfs:isDefinedBy <https://w3id.org/seas/BuildingOntology> ;
                     rdfs:label "HolidayBuilding"@en ,
                                "VapaaAjanRakennus"@fi ;
                     vs:term_status "testing" .


###  https://w3id.org/seas/HomeOffice
seas:HomeOffice rdf:type owl:Class ;
                rdfs:subClassOf seas:Office ;
                rdfs:comment "A work or office space set up in a person's home and used exclusively for business on a regular basis."@en ;
                rdfs:isDefinedBy <https://w3id.org/seas/BuildingOntology> ;
                rdfs:label "Tree house"@en ;
                vs:term_status "testing" .


###  https://w3id.org/seas/IndustrialBuilding
seas:IndustrialBuilding rdf:type owl:Class ;
                        rdfs:subClassOf seas:NonResidentalBuilding ;
                        rdfs:comment "Buildings used for industrial production, e.g. factories, workshops, slaughterhouses, breweries, assembly plants, etc."@en ;
                        rdfs:isDefinedBy <https://w3id.org/seas/BuildingOntology> ;
                        rdfs:label "IndustrialBuilding"@en ;
                        vs:term_status "testing" .


###  https://w3id.org/seas/InstitutionalBuilding
seas:InstitutionalBuilding rdf:type owl:Class ;
                           rdfs:subClassOf seas:NonResidentalBuilding ;
                           rdfs:comment "Institutions such as hospitals providing medical and surgical treatment and nursing care for ill or injured people."@en ;
                           rdfs:isDefinedBy <https://w3id.org/seas/BuildingOntology> ;
                           rdfs:label "HoitoalanRakennus"@fi ,
                                      "InstitutionalBuilding"@en ;
                           vs:term_status "testing" .


###  https://w3id.org/seas/Kitchen
seas:Kitchen rdf:type owl:Class ;
             rdfs:subClassOf seas:Room ;
             rdfs:comment "Kitchen is a room used mainly for cooking and possibly eating."@en ;
             rdfs:isDefinedBy <https://w3id.org/seas/BuildingOntology> ;
             rdfs:label "Kitchen"@en ;
             vs:term_status "testing" .


###  https://w3id.org/seas/Laundry
seas:Laundry rdf:type owl:Class ;
             rdfs:subClassOf seas:Room ;
             rdfs:comment "A room or zone, as in a home or apartment building, reserved for doing the family wash."@en ;
             rdfs:isDefinedBy <https://w3id.org/seas/BuildingOntology> ;
             rdfs:label "Laundry"@en ;
             vs:term_status "testing" .


###  https://w3id.org/seas/LivingRoom
seas:LivingRoom rdf:type owl:Class ;
                rdfs:subClassOf seas:Room ;
                rdfs:comment "Living Room is the main room of daytime activity."@en ;
                rdfs:isDefinedBy <https://w3id.org/seas/BuildingOntology> ;
                rdfs:label "Living Room"@en ;
                vs:term_status "testing" .


###  https://w3id.org/seas/Lobby
seas:Lobby rdf:type owl:Class ;
           rdfs:subClassOf seas:Room ;
           rdfs:comment "An entrance hall, corridor, or vestibule, as in a public building, often serving as an anteroom; foyer."@en ;
           rdfs:isDefinedBy <https://w3id.org/seas/BuildingOntology> ;
           rdfs:label "Lobby"@en ;
           vs:term_status "testing" .


###  https://w3id.org/seas/LowEnergyHouse
seas:LowEnergyHouse rdf:type owl:Class ;
                    rdfs:subClassOf seas:Building ;
                    rdfs:comment "A house typically consuming half the energy than a norm house."@en ;
                    rdfs:isDefinedBy <https://w3id.org/seas/BuildingOntology> ;
                    rdfs:label "LowEnergyHouse"@en ,
                               "Matalaenergiatalo"@fi ;
                    vs:term_status "testing" .


###  https://w3id.org/seas/MercantileBuilding
seas:MercantileBuilding rdf:type owl:Class ;
                        rdfs:subClassOf seas:NonResidentalBuilding ;
                        rdfs:comment "Places where goods are displayed and sold. Examples: grocery stores, department stores, and gas stations."@en ;
                        rdfs:isDefinedBy <https://w3id.org/seas/BuildingOntology> ;
                        rdfs:label "Liikerakennus"@fi ,
                                   "MercantileBuilding"@en ;
                        vs:term_status "testing" .


###  https://w3id.org/seas/NonResidentalBuilding
seas:NonResidentalBuilding rdf:type owl:Class ;
                           rdfs:subClassOf seas:Building ;
                           rdfs:comment "A  non-residential building is a building at least half of which is used for other than residential purposes. "@en ;
                           rdfs:isDefinedBy <https://w3id.org/seas/BuildingOntology> ;
                           rdfs:label "NonResidentalBuilding"@en ;
                           vs:term_status "testing" .


###  https://w3id.org/seas/NormHouse
seas:NormHouse rdf:type owl:Class ;
               rdfs:subClassOf seas:Building ;
               rdfs:comment "A building fulfilling the minimal criteria for energy efficiency."@en ;
               rdfs:isDefinedBy <https://w3id.org/seas/BuildingOntology> ;
               rdfs:label "NormHouse"@en ,
                          "Normitalo"@fi ;
               vs:term_status "testing" .


###  https://w3id.org/seas/Office
seas:Office rdf:type owl:Class ;
            rdfs:subClassOf seas:Room ;
            rdfs:comment "A room, set of rooms, or building where the business of a commercial or industrial organization or of a professional person is conducted."@en ;
            rdfs:isDefinedBy <https://w3id.org/seas/BuildingOntology> ;
            rdfs:label "Office"@en ;
            vs:term_status "testing" .


###  https://w3id.org/seas/OfficeBuilding
seas:OfficeBuilding rdf:type owl:Class ;
                    rdfs:subClassOf seas:NonResidentalBuilding ;
                    rdfs:comment "Places where services are provided. Examples: banks, insurance agencies."@en ;
                    rdfs:isDefinedBy <https://w3id.org/seas/BuildingOntology> ;
                    rdfs:label "BusinessBuilding"@en ,
                               "Toimistorakennus"@fi ;
                    vs:term_status "testing" .


###  https://w3id.org/seas/OneDwellingBuilding
seas:OneDwellingBuilding rdf:type owl:Class ;
                         rdfs:subClassOf seas:SmallHouse ;
                         rdfs:comment "Detached house."@en ;
                         rdfs:isDefinedBy <https://w3id.org/seas/BuildingOntology> ;
                         rdfs:label "OneDwellingBuilding"@en ,
                                    "YhdenAsunnonTalo"@fi ;
                         vs:term_status "testing" .


###  https://w3id.org/seas/OpenBuildingSpaceConnection
seas:OpenBuildingSpaceConnection rdf:type owl:Class ;
                                 rdfs:subClassOf seas:BuildingSpaceConnection ;
                                 owl:disjointWith seas:OpennableBuildingSpaceConnection ;
                                 rdfs:comment """An open building space connection is a connection between two building spaces that is open.

  This connection may for instance be a hole in a wall, or a virtual separation between two offices in an open space.

  Instances of `seas:OpenBuildingSpaceConnection` may be typed by classes from specialized building ontologies."""@en ;
                                 rdfs:isDefinedBy <https://w3id.org/seas/BuildingOntology> ;
                                 rdfs:label "Open Building Space Connection"@en ;
                                 vs:term_status "testing" .


###  https://w3id.org/seas/OpennableBuildingSpaceConnection
seas:OpennableBuildingSpaceConnection rdf:type owl:Class ;
                                      rdfs:subClassOf seas:BuildingSpaceConnection ;
                                      rdfs:comment """An opennable building space connection is a connection between two building spaces that has a certain degree of openness.

  This connection may for instance be a window or a door.

  Instances of `seas:OpennableBuildingSpaceConnection` may be typed by classes from specialized building ontologies."""@en ;
                                      rdfs:isDefinedBy <https://w3id.org/seas/BuildingOntology> ;
                                      rdfs:label "Opennable Building Space Connection"@en ;
                                      vs:term_status "testing" .


###  https://w3id.org/seas/PassiveHouse
seas:PassiveHouse rdf:type owl:Class ;
                  rdfs:subClassOf seas:Building ;
                  rdfs:comment "A house typically consuming a quarter of the energy than a norm house."@en ;
                  rdfs:isDefinedBy <https://w3id.org/seas/BuildingOntology> ;
                  rdfs:label "Passiivitalo"@fi ,
                             "PassiveHouse"@en ;
                  vs:term_status "testing" .


###  https://w3id.org/seas/PlusEnergyBuilding
seas:PlusEnergyBuilding rdf:type owl:Class ;
                        rdfs:subClassOf seas:Building ;
                        rdfs:comment "A net plus-energy building is a building that over a year does generates more energy than it uses. "@en ;
                        rdfs:isDefinedBy <https://w3id.org/seas/BuildingOntology> ;
                        rdfs:label "PlusEnergyBuilding"@en ,
                                   "Plusenergiatalo"@fi ;
                        vs:term_status "testing" .


###  https://w3id.org/seas/PowerplantBuilding
seas:PowerplantBuilding rdf:type owl:Class ;
                        rdfs:subClassOf seas:IndustrialBuilding ;
                        rdfs:comment "Places housing any type of a power plants."@en ;
                        rdfs:isDefinedBy <https://w3id.org/seas/BuildingOntology> ;
                        rdfs:label "PowerplantBuilding"@en ,
                                   "VoimalaRakennus"@fi ;
                        vs:term_status "testing" .


###  https://w3id.org/seas/ResidentalBuilding
seas:ResidentalBuilding rdf:type owl:Class ;
                        rdfs:subClassOf seas:Building ;
                        rdfs:comment "A residential building is a building at least half of which is used for residential purposes. "@en ;
                        rdfs:isDefinedBy <https://w3id.org/seas/BuildingOntology> ;
                        rdfs:label "Asuinrakennus"@fi ,
                                   "ResidentalBuilding"@en ;
                        vs:term_status "testing" .


###  https://w3id.org/seas/Roof
seas:Roof rdf:type owl:Class ;
          rdfs:subClassOf seas:BuildingSpaceConnection ;
          rdfs:comment "A (tilted more than 60 percent) vertical surface that separates building spaces."@en ;
          rdfs:isDefinedBy <https://w3id.org/seas/BuildingOntology> ;
          rdfs:label "Roof"@en ;
          vs:term_status "testing" .


###  https://w3id.org/seas/Room
seas:Room rdf:type owl:Class ;
          rdfs:subClassOf seas:BuildingSpace ;
          rdfs:comment "A room in a building space enclosed by surfaces, this could also be modelled as role of space, not subclass of the space itself."@en ;
          rdfs:isDefinedBy <https://w3id.org/seas/BuildingOntology> ;
          rdfs:label "Room"@en ;
          vs:term_status "testing" .


###  https://w3id.org/seas/Sauna
seas:Sauna rdf:type owl:Class ;
           rdfs:subClassOf seas:Room ;
           rdfs:comment "Sauna is a special type bathroom for enjoying hot dry air."@en ;
           rdfs:isDefinedBy <https://w3id.org/seas/BuildingOntology> ;
           rdfs:label "Sauna"@en ;
           vs:term_status "testing" .


###  https://w3id.org/seas/SiteOfBuilding
seas:SiteOfBuilding rdf:type owl:Class ;
                    rdfs:subClassOf seas:Zone ;
                    rdfs:comment "Building site is a locale containing one or more separate buildings. They are zones."@en ;
                    rdfs:isDefinedBy <https://w3id.org/seas/BuildingOntology> ;
                    rdfs:label "SiteOfBuilding"@en ;
                    vs:term_status "testing" .


###  https://w3id.org/seas/SmallHouse
seas:SmallHouse rdf:type owl:Class ;
                rdfs:subClassOf seas:ResidentalBuilding ;
                rdfs:comment "A detached small residential building."@en ;
                rdfs:isDefinedBy <https://w3id.org/seas/BuildingOntology> ;
                rdfs:label "Pientalo"@en ,
                           "SmallHouse"@en ;
                vs:term_status "testing" .


###  https://w3id.org/seas/Stairs
seas:Stairs rdf:type owl:Class ;
            rdfs:subClassOf seas:BuildingSpace ;
            rdfs:comment "A construction designed to bridge a large vertical distance by dividing it into smaller vertical distances, called steps."@en ;
            rdfs:isDefinedBy <https://w3id.org/seas/BuildingOntology> ;
            rdfs:label "Stairs"@en ;
            vs:term_status "testing" .


###  https://w3id.org/seas/StorageBuilding
seas:StorageBuilding rdf:type owl:Class ;
                     rdfs:subClassOf seas:NonResidentalBuilding ;
                     rdfs:comment "Places where items are stored. Examples: warehouses, reservoirs and silos."@en ;
                     rdfs:isDefinedBy <https://w3id.org/seas/BuildingOntology> ;
                     rdfs:label "StorageBuilding"@en ,
                                "VarastoRakennus"@fi ;
                     vs:term_status "testing" .


###  https://w3id.org/seas/StorageRoom
seas:StorageRoom rdf:type owl:Class ;
                 rdfs:subClassOf seas:Room ;
                 rdfs:comment "Room for storage."@en ;
                 rdfs:isDefinedBy <https://w3id.org/seas/BuildingOntology> ;
                 rdfs:label "Storage Room"@en ;
                 vs:term_status "testing" .


###  https://w3id.org/seas/Sunroom
seas:Sunroom rdf:type owl:Class ;
             rdfs:subClassOf seas:Room ;
             rdfs:comment "A structure, either attached or integrated into a building, which allows enjoyment of the surrounding landscape while being sheltered from adverse weather."@en ;
             rdfs:isDefinedBy <https://w3id.org/seas/BuildingOntology> ;
             rdfs:label "Swimming Pool"@en ;
             vs:term_status "testing" .


###  https://w3id.org/seas/SwimmingPool
seas:SwimmingPool rdf:type owl:Class ;
                  rdfs:subClassOf seas:BuildingSpace ;
                  rdfs:comment "A tank or large artificial basin, as of concrete, for filling with water for swimming."@en ;
                  rdfs:isDefinedBy <https://w3id.org/seas/BuildingOntology> ;
                  rdfs:label "Swimming Pool"@en ;
                  vs:term_status "testing" .


###  https://w3id.org/seas/TreeHouse
seas:TreeHouse rdf:type owl:Class ;
               rdfs:subClassOf seas:BuildingSpace ;
               rdfs:comment "A small house, especially one for children to play in, built or placed up in the branches of a tree."@en ;
               rdfs:isDefinedBy <https://w3id.org/seas/BuildingOntology> ;
               rdfs:label "Tree House"@en ;
               vs:term_status "testing" .


###  https://w3id.org/seas/UtilityRoom
seas:UtilityRoom rdf:type owl:Class ;
                 rdfs:subClassOf seas:Room ;
                 rdfs:comment "Room for other special utilities and hobbies."@en ;
                 rdfs:isDefinedBy <https://w3id.org/seas/BuildingOntology> ;
                 rdfs:label "Utility Room"@en ;
                 vs:term_status "testing" .


###  https://w3id.org/seas/Wall
seas:Wall rdf:type owl:Class ;
          rdfs:subClassOf seas:BuildingSpaceConnection ;
          rdfs:comment "A roof upwards tilted surface tilted up part of upper envelope of building."@en ;
          rdfs:isDefinedBy <https://w3id.org/seas/BuildingOntology> ;
          rdfs:label "Wall"@en ;
          vs:term_status "testing" .


###  https://w3id.org/seas/Window
seas:Window rdf:type owl:Class ;
            rdfs:subClassOf seas:BuildingSpaceConnection ;
            rdfs:comment "a space or an zone of glass in the wall of a building or vehicle that lets in light (Longman Dictionary of Contemporary English Online)"@en ;
            rdfs:isDefinedBy <https://w3id.org/seas/BuildingOntology> ;
            rdfs:label "Window"@en ;
            vs:term_status "testing" .


###  https://w3id.org/seas/Yard
seas:Yard rdf:type owl:Class ;
          rdfs:subClassOf seas:BuildingSpace ;
          rdfs:comment "A small usually walled and often paved zone open to the sky and adjacent to a building."@en ;
          rdfs:isDefinedBy <https://w3id.org/seas/BuildingOntology> ;
          rdfs:label "Yard"@en ;
          vs:term_status "testing" .


###  https://w3id.org/seas/ZeroEnergyBuilding
seas:ZeroEnergyBuilding rdf:type owl:Class ;
                        rdfs:subClassOf seas:Building ;
                        rdfs:comment "A net zero-energy building (ZEB) is a building that over a year does not use more energy than it generates. "@en ;
                        rdfs:isDefinedBy <https://w3id.org/seas/BuildingOntology> ;
                        rdfs:label "Nollaenergiatalo"@fi ,
                                   "ZeroEnergyBuilding"@en ;
                        vs:term_status "testing" .


#################################################################
#    Individuals
#################################################################

###  https://w3id.org/seas/BuildingOntology
<https://w3id.org/seas/BuildingOntology> rdf:type owl:NamedIndividual ,
                                                  voaf:Vocabulary .


[ rdf:type foaf:Person ;
  foaf:name "Gabriel Santos"
] .

[ rdf:type foaf:Person ;
   foaf:name "Francisco Silva"
 ] .

[ rdf:type foaf:Person ;
   foaf:name "Brigida Teixeira"
 ] .

###  Generated by the OWL API (version 4.2.8.20170104-2310) https://github.com/owlcs/owlapi
