# Copyright 2016 ITEA 12004 SEAS Project.
# 
# Licensed under the Apache License, Version 2.0 (the "License");
# you may not use this file except in compliance with the License.
# You may obtain a copy of the License at
# 
#      http://www.apache.org/licenses/LICENSE-2.0
# 
# Unless required by applicable law or agreed to in writing,
# distributed under the License is distributed on an "AS IS" BASIS,
# WITHOUT WARRANTIES OR CONDITIONS OF ANY KIND, either express or implied.
# See the License for the specific language governing permissions and
# limitations under the License.

@prefix rdf: <http://www.w3.org/1999/02/22-rdf-syntax-ns#> .
@prefix owl: <http://www.w3.org/2002/07/owl#> .
@prefix rdfs: <http://www.w3.org/2000/01/rdf-schema#> .
@prefix xsd: <http://www.w3.org/2001/XMLSchema#> .
@prefix dcterms: <http://purl.org/dc/terms/> .
@prefix vann: <http://purl.org/vocab/vann/> .
@prefix voaf: <http://purl.org/vocommons/voaf#> .
@prefix vs: <http://www.w3.org/2003/06/sw-vocab-status/ns#> .
@prefix cc: <http://creativecommons.org/ns#>.
@prefix foaf: <http://xmlns.com/foaf/0.1/>.
@prefix saref: <http://ontology.tno.nl/saref#>. #SAREF smart building appliances ontology
@prefix qudt: <http://data.qudt.org/qudt/owl/1.0.0/qudt.owl#> .
@prefix qudt-unit: <http://data.qudt.org/qudt/owl/1.0.0/unit.owl#> . #QUDT units
@prefix ssn: <http://www.w3.org/ns/ssn/>.
@prefix skos: <http://www.w3.org/2004/02/skos/core#>.
@prefix sdmx: <http://purl.org/linked-data/sdmx#>.

@prefix seas: <https://w3id.org/seas/>.
@base <https://w3id.org/seas/>.

voaf:Vocabulary a owl:Class .
dcterms:title a owl:AnnotationProperty .
dcterms:description a owl:AnnotationProperty .
dcterms:issued a owl:AnnotationProperty .
dcterms:modified a owl:AnnotationProperty .
dcterms:creator a owl:AnnotationProperty .
dcterms:contributor a owl:AnnotationProperty .
cc:license a owl:AnnotationProperty .
vann:preferredNamespacePrefix a owl:AnnotationProperty .
vann:preferredNamespaceUri a owl:AnnotationProperty .
vs:term_status a owl:AnnotationProperty .
foaf:Person a owl:Class .
foaf:name a owl:DatatypeProperty .


seas:CommunicationOntology rdf:type voaf:Vocabulary , owl:Ontology ;
  dcterms:title "The SEAS Communication ontology"@en ;
  dcterms:description """The SEAS Communication ontology defines:

1. Communication devices that ca connect to exchange information,
2. Communication connections between Communication devices, where information is exchanged, and
3. Communication connection points of communication devices, through which information flows in/out the communication device."""@en ;
  dcterms:issued "2017-03-13"^^xsd:date ;
  dcterms:modified "2017-03-13"^^xsd:date ;
  dcterms:creator <http://www.maxime-lefrancois.info/me#> ;
  cc:license <https://www.apache.org/licenses/LICENSE-2.0> ;
  vann:preferredNamespacePrefix "seas" ;
  vann:preferredNamespaceUri <https://w3id.org/seas/> ;  
  owl:imports seas:DeviceOntology ;
  owl:versionIRI <https://w3id.org/seas/CommunicationOntology-1.0> ;
  owl:versionInfo "v1.0" .

## communication device

seas:CommunicationDevice a owl:Class ;
  rdfs:label "Communication Device"@en ;
  rdfs:comment """The class of communication devices, i.e., devices that exchange information with other communication devices.

  These exchange are only possible through information connections between communication devices."""@en ;
  rdfs:subClassOf seas:Device ;
  vs:term_status "testing" ;
  rdfs:isDefinedBy seas:CommunicationOntology .

  seas:WireCommunicationDevice a owl:Class ;
    rdfs:label "Wire Communication Device"@en ;
    rdfs:comment """The class of communication devices capable of communicating through a wire.

    SEAS defines a taxonomy of communication devices used by SEAS partners. If another user requires some addition to this list, please contact us."""@en ;
    rdfs:subClassOf seas:CommunicationDevice ;
    owl:equivalentClass [ owl:onProperty seas:connectsAt ; owl:someValuesFrom  seas:WireCommunicationConnectionPoint ] ;
    vs:term_status "testing" ;
    rdfs:isDefinedBy seas:CommunicationOntology .

    seas:SerialCommunicationDevice a owl:Class ;
      rdfs:label "Serial Communication Device"@en ;
      rdfs:comment """The class of communication devices capable of communicating using the serial protocol."""@en ;
      rdfs:subClassOf seas:WireCommunicationDevice ;
      owl:equivalentClass [ owl:onProperty seas:connectsAt ; owl:someValuesFrom  seas:SerialCommunicationConnectionPoint ] ;
      vs:term_status "testing" ;
      rdfs:isDefinedBy seas:CommunicationOntology .

    seas:USBCommunicationDevice a owl:Class ;
      rdfs:label "USB Communication Device"@en ;
      rdfs:comment """The class of communication devices capable of communicating using the USB protocol."""@en ;
      rdfs:subClassOf seas:WireCommunicationDevice ;
      owl:equivalentClass [ owl:onProperty seas:connectsAt ; owl:someValuesFrom  seas:USBCommunicationConnectionPoint ] ;
      vs:term_status "testing" ;
      rdfs:isDefinedBy seas:CommunicationOntology .

  seas:WirelessCommunicationDevice a owl:Class ;
    rdfs:label "Wireless Communication Device"@en ;
    rdfs:comment """The class of communication devices capable of communicating wirelessly."""@en ;
    rdfs:subClassOf seas:CommunicationDevice ;
    owl:equivalentClass [ owl:onProperty seas:connectsAt ; owl:someValuesFrom  seas:WirelessCommunicationConnectionPoint ] ;
    vs:term_status "testing" ;
    rdfs:isDefinedBy seas:CommunicationOntology .

    seas:RadioCommunicationDevice a owl:Class ;
      rdfs:label "Radio Communication Device"@en ;
      rdfs:comment """The class of communication devices capable of communicating using radio waves."""@en ;
      rdfs:subClassOf seas:WirelessCommunicationDevice ;
      owl:equivalentClass [ owl:onProperty seas:connectsAt ; owl:someValuesFrom  seas:RadioCommunicationConnectionPoint ] ;
      vs:term_status "testing" ;
      rdfs:isDefinedBy seas:CommunicationOntology .

      seas:SigFoxCommunicationDevice a owl:Class ;
        rdfs:label "SigFox Communication Device"@en ;
        rdfs:comment """The class of communication devices capable of communicating using the SigFox protocol."""@en ;
        rdfs:subClassOf seas:RadioCommunicationDevice ;
        owl:equivalentClass [ owl:onProperty seas:connectsAt ; owl:someValuesFrom  seas:SigFoxCommunicationConnectionPoint ] ;
        vs:term_status "testing" ;
        rdfs:isDefinedBy seas:CommunicationOntology .

      seas:ZigBeeCommunicationDevice a owl:Class ;
        rdfs:label "ZigBee Communication Device"@en ;
        rdfs:comment """The class of communication devices capable of communicating using the ZigBee protocol."""@en ;
        rdfs:subClassOf seas:RadioCommunicationDevice ;
        owl:equivalentClass [ owl:onProperty seas:connectsAt ; owl:someValuesFrom  seas:ZigBeeCommunicationConnectionPoint ] ;
        vs:term_status "testing" ;
        rdfs:isDefinedBy seas:CommunicationOntology .

      seas:LoRaCommunicationDevice a owl:Class ;
        rdfs:label "LoRa Communication Device"@en ;
        rdfs:comment """The class of communication devices capable of communicating using the LoRa protocol."""@en ;
        rdfs:subClassOf seas:RadioCommunicationDevice ;
        owl:equivalentClass [ owl:onProperty seas:connectsAt ; owl:someValuesFrom  seas:LoRaCommunicationConnectionPoint ] ;
        vs:term_status "testing" ;
        rdfs:isDefinedBy seas:CommunicationOntology .

      seas:BLECommunicationDevice a owl:Class ;
        rdfs:label "BLE Communication Device"@en ;
        rdfs:comment """The class of communication devices capable of communicating using the BLE protocol."""@en ;
        rdfs:subClassOf seas:RadioCommunicationDevice ;
        owl:equivalentClass [ owl:onProperty seas:connectsAt ; owl:someValuesFrom  seas:BLECommunicationConnectionPoint ] ;
        vs:term_status "testing" ;
        rdfs:isDefinedBy seas:CommunicationOntology .

      seas:BluetoothCommunicationDevice a owl:Class ;
        rdfs:label "Bluetooth Communication Device"@en ;
        rdfs:comment """The class of communication devices capable of communicating using the Bluetooth protocol."""@en ;
        rdfs:subClassOf seas:RadioCommunicationDevice ;
        owl:equivalentClass [ owl:onProperty seas:connectsAt ; owl:someValuesFrom  seas:BluetoothCommunicationConnectionPoint ] ;
        vs:term_status "testing" ;
        rdfs:isDefinedBy seas:CommunicationOntology .

      seas:WiFiCommunicationDevice a owl:Class ;
        rdfs:label "WiFi Communication Device"@en ;
        rdfs:comment """The class of communication devices capable of communicating using the WiFi protocol."""@en ;
        rdfs:subClassOf seas:RadioCommunicationDevice ;
        owl:equivalentClass [ owl:onProperty seas:connectsAt ; owl:someValuesFrom  seas:WiFiCommunicationConnectionPoint ] ;
        vs:term_status "testing" ;
        rdfs:isDefinedBy seas:CommunicationOntology .

      seas:EnOceanCommunicationDevice a owl:Class ;
        rdfs:label "EnOcean Communication Device"@en ;
        rdfs:comment """The class of communication devices capable of communicating using the EnOcean protocol."""@en ;
        rdfs:subClassOf seas:RadioCommunicationDevice ;
        owl:equivalentClass [ owl:onProperty seas:connectsAt ; owl:someValuesFrom  seas:EnOceanCommunicationConnectionPoint ] ;
        vs:term_status "testing" ;
        rdfs:isDefinedBy seas:CommunicationOntology .


seas:communicatesWith a owl:ObjectProperty , owl:SymmetricProperty ;
  rdfs:label "communicates with"@en ;
  rdfs:comment """Links a communication device to another communication device it exchanges information with. 

  For example, for information to flow between a water smart meter and a smart home management system, then they must share a communication connection:

```
  <waterSmartMeter> a seas:CommunicationDevice .
  <smartHMS> a seas:CommunicationDevice .
  <waterSmartMeter> seas:communicatesWith <smartHMS> . 
```

  This property can be further specialized to describe the communication protocol used. For example, sub property `seas:communicatesIn80211aWith` links a communication device to another communication device it exchanges information with using WiFi 802.11a norm.

  This property can be qualified using class seas:CommunicationConnection, which connects (at least) the two communication systems.
  If there is a communication connection between several communication devices, then one may infer these communication devices can exchange information.

    SEAS defines a some communicatesWith sub properties used by SEAS partners. If another user requires some addition to this list, please contact us."""@en ;
  rdfs:subPropertyOf seas:connectedTo ;
  rdfs:domain seas:CommunicationDevice ;
  rdfs:range seas:CommunicationDevice ;
  vs:term_status "testing" ;
  rdfs:isDefinedBy seas:CommunicationOntology .

  seas:communicatesUsingWireWith a owl:ObjectProperty , owl:SymmetricProperty ;
    rdfs:label "communicates using wire with"@en;
    rdfs:comment """Links a communication device to another communication device it exchanges information with using some wire."""@en;
    rdfs:subPropertyOf seas:communicatesWith;
    vs:term_status "unstable"  ;
    rdfs:isDefinedBy seas:SmartMeterOntology .

    seas:communicatesInSerialWith a owl:ObjectProperty , owl:SymmetricProperty ;
      rdfs:label "communicates in Serial With"@en;
      rdfs:comment """Links a communication device to another communication device it exchanges information with using Serial protocol."""@en;
      rdfs:subPropertyOf seas:communicatesUsingWireWith;
      vs:term_status "unstable"  ;
      rdfs:isDefinedBy seas:SmartMeterOntology .  

    seas:communicatesInUSBWith a owl:ObjectProperty , owl:SymmetricProperty ;
      rdfs:label "communicates in USB With"@en;
      rdfs:comment """Links a communication device to another communication device it exchanges information with using USB protocol."""@en;
      rdfs:subPropertyOf seas:communicatesUsingWireWith;
      vs:term_status "unstable"  ;
      rdfs:isDefinedBy seas:SmartMeterOntology .  

  seas:communicatesWirelesslyWith a owl:ObjectProperty , owl:SymmetricProperty ;
    rdfs:label "communicates wirelessly with"@en;
    rdfs:comment """Links a communication device to another communication device it exchanges information with wirelessly."""@en;
    rdfs:subPropertyOf seas:communicatesWith;
    vs:term_status "unstable"  ;
    rdfs:isDefinedBy seas:SmartMeterOntology .  

    seas:communicatesInRadioWith a owl:ObjectProperty , owl:SymmetricProperty ;
      rdfs:label "communicates in Radio With"@en;
      rdfs:comment """Links a communication device to another communication device it exchanges information with using Radio Waves."""@en;
      rdfs:subPropertyOf seas:communicatesWirelesslyWith;
      vs:term_status "unstable"  ;
      rdfs:isDefinedBy seas:SmartMeterOntology .  

      seas:communicatesInSigFoxWith a owl:ObjectProperty , owl:SymmetricProperty ;
        rdfs:label "communicates in SigFox With"@en;
        rdfs:comment """Links a communication device to another communication device it exchanges information with using the SigFox protocol."""@en;
        rdfs:subPropertyOf seas:communicatesInRadioWith;
        vs:term_status "unstable"  ;
        rdfs:isDefinedBy seas:SmartMeterOntology .  

      seas:communicatesInZigBeeWith a owl:ObjectProperty , owl:SymmetricProperty ;
        rdfs:label "communicates in Zig Bee With"@en;
        rdfs:comment """Links a communication device to another communication device it exchanges information with using the Zig Bee protocol."""@en;
        rdfs:subPropertyOf seas:communicatesInRadioWith;
        vs:term_status "unstable"  ;
        rdfs:isDefinedBy seas:SmartMeterOntology .  

      seas:communicatesInLoRaWith a owl:ObjectProperty , owl:SymmetricProperty ;
        rdfs:label "communicates in LoRa With"@en;
        rdfs:comment """Links a communication device to another communication device it exchanges information with using the LoRa protocol."""@en;
        rdfs:subPropertyOf seas:communicatesInRadioWith;
        vs:term_status "unstable"  ;
        rdfs:isDefinedBy seas:SmartMeterOntology .  

      seas:communicatesInBLEWith a owl:ObjectProperty , owl:SymmetricProperty ;
        rdfs:label "communicates in BLE With"@en;
        rdfs:comment """Links a communication device to another communication device it exchanges information with using the Bluetooth Low Energy protocol."""@en;
        rdfs:subPropertyOf seas:communicatesInRadioWith;
        vs:term_status "unstable"  ;
        rdfs:isDefinedBy seas:SmartMeterOntology .  

      seas:communicatesInBluetoothWith a owl:ObjectProperty , owl:SymmetricProperty ;
        rdfs:label "communicates in Bluetooth With"@en;
        rdfs:comment """Links a communication device to another communication device it exchanges information with using the Bluetooth protocol."""@en;
        rdfs:subPropertyOf seas:communicatesInRadioWith;
        vs:term_status "unstable"  ;
        rdfs:isDefinedBy seas:SmartMeterOntology .  

      seas:communicatesInWifiWith a owl:ObjectProperty , owl:SymmetricProperty ;
        rdfs:label "communicates in Wifi With"@en;
        rdfs:comment """Links a communication device to another communication device it exchanges information with using the Wifi protocol."""@en;
        rdfs:subPropertyOf seas:communicatesInRadioWith;
        vs:term_status "unstable"  ;
        rdfs:isDefinedBy seas:SmartMeterOntology .  

      seas:communicatesInEnOceanWith a owl:ObjectProperty , owl:SymmetricProperty ;
        rdfs:label "communicates in EnOcean With"@en;
        rdfs:comment """Links a communication device to another communication device it exchanges information with using the EnOcean protocol."""@en;
        rdfs:subPropertyOf seas:communicatesInRadioWith;
        vs:term_status "unstable"  ;
        rdfs:isDefinedBy seas:SmartMeterOntology .  

      # ...


## communication connection

seas:CommunicationConnection a owl:Class ;
  rdfs:label "Communication Connection"@en ;
  rdfs:comment """The class of communication connections between communication devices.
  a communication connection describes the information flows between the communication devices it connects.
  For example, the following RDF graph states that a 802.11a (WiFi) connection connects two :

```
  <wifi_connection_12> a seas:CommunicationConnection ;
    seas:connectsSystem <waterSmartMeter> , <smartHMS> .
```

  Only communication devices and communication connection points are connected through a communication connection.
  A connection between communication devices is not necessarily a communication connection.

  Any communication device that exchanges information through a communication connection is connected at least through one of its communication connection points to the communication connection:
  if:

```
  <waterSmartMeter> a seas:CommunicationDevice .
  <wifi_connection_12> a seas:CommunicationConnection .
  <waterSmartMeter> seas:connectedThrough <wifi_connection_12> .
```

  then there exists `_:communicationConnectionPoint` such that:

```
  _:communicationConnectionPoint a seas:CommunicationConnectionPoint ;
    seas:connectionPointOf <waterSmartMeter> ;
    seas:connectsSystemThrough <wifi_connection_12> .
```

    SEAS defines a taxonomy of communication connections used by SEAS partners. If another user requires some addition to this list, please contact us.
"""@en ;
  rdfs:subClassOf seas:Connection ;
  rdfs:subClassOf [ owl:onProperty seas:connectsSystem ; owl:allValuesFrom  seas:CommunicationDevice ] ;
  rdfs:subClassOf [ owl:onProperty seas:connectsSystemAt ; owl:allValuesFrom  seas:CommunicationConnectionPoint ] ;
  vs:term_status "testing" ;
  rdfs:isDefinedBy seas:CommunicationOntology .

  seas:WireCommunicationConnection a owl:Class ;
    rdfs:label "Wire Communication Connection"@en ;
    rdfs:comment """The class of wire communication connections between communication devices."""@en ;
    rdfs:subClassOf seas:CommunicationConnection ;
    rdfs:subClassOf [ owl:onProperty seas:connectsSystem ; owl:allValuesFrom  seas:WireCommunicationDevice ] ;
    rdfs:subClassOf [ owl:onProperty seas:connectsSystemAt ; owl:allValuesFrom  seas:WireCommunicationConnectionPoint ] ;
    vs:term_status "testing" ;
    rdfs:isDefinedBy seas:CommunicationOntology .
      
    seas:SerialCommunicationConnection a owl:Class ;
      rdfs:label "Serial Communication Connection"@en ;
      rdfs:comment """The class of Serial communication connections between communication devices."""@en ;
      rdfs:subClassOf seas:WireCommunicationConnection ;
      rdfs:subClassOf [ owl:onProperty seas:connectsSystem ; owl:allValuesFrom  seas:SerialCommunicationDevice ] ;
      rdfs:subClassOf [ owl:onProperty seas:connectsSystemAt ; owl:allValuesFrom  seas:SerialCommunicationConnectionPoint ] ;
      vs:term_status "testing" ;
      rdfs:isDefinedBy seas:CommunicationOntology .

    seas:USBCommunicationConnection a owl:Class ;
      rdfs:label "USB Communication Connection"@en ;
      rdfs:comment """The class of USB communication connections between communication devices."""@en ;
      rdfs:subClassOf seas:WireCommunicationConnection ;
      rdfs:subClassOf [ owl:onProperty seas:connectsSystem ; owl:allValuesFrom  seas:USBCommunicationDevice ] ;
      rdfs:subClassOf [ owl:onProperty seas:connectsSystemAt ; owl:allValuesFrom  seas:USBCommunicationConnectionPoint ] ;
      vs:term_status "testing" ;
      rdfs:isDefinedBy seas:CommunicationOntology .

  seas:WirelessCommunicationConnection a owl:Class ;
    rdfs:label "Wireless Communication Connection"@en ;
    rdfs:comment """The class of wireless communication connections between communication devices."""@en ;
    rdfs:subClassOf seas:CommunicationConnection ;
    rdfs:subClassOf [ owl:onProperty seas:connectsSystem ; owl:allValuesFrom  seas:WirelessCommunicationDevice ] ;
    rdfs:subClassOf [ owl:onProperty seas:connectsSystemAt ; owl:allValuesFrom  seas:WirelessCommunicationConnectionPoint ] ;
    vs:term_status "testing" ;
    rdfs:isDefinedBy seas:CommunicationOntology .

    seas:RadioCommunicationConnection a owl:Class ;
      rdfs:label "Radio Communication Connection"@en ;
      rdfs:comment """The class of radio communication connections between communication devices."""@en ;
      rdfs:subClassOf seas:WirelessCommunicationConnection ;
      rdfs:subClassOf [ owl:onProperty seas:connectsSystem ; owl:allValuesFrom  seas:RadioCommunicationDevice ] ;
      rdfs:subClassOf [ owl:onProperty seas:connectsSystemAt ; owl:allValuesFrom  seas:RadioCommunicationConnectionPoint ] ;
      vs:term_status "testing" ;
      rdfs:isDefinedBy seas:CommunicationOntology .

      seas:SigFoxCommunicationConnection a owl:Class ;
        rdfs:label "SigFox Communication Connection"@en ;
        rdfs:comment """The class of SigFox communication connections between communication devices."""@en ;
        rdfs:subClassOf seas:RadioCommunicationConnection ;
        rdfs:subClassOf [ owl:onProperty seas:connectsSystem ; owl:allValuesFrom  seas:SigFoxCommunicationDevice ] ;
        rdfs:subClassOf [ owl:onProperty seas:connectsSystemAt ; owl:allValuesFrom  seas:SigFoxCommunicationConnectionPoint ] ;
        vs:term_status "testing" ;
        rdfs:isDefinedBy seas:CommunicationOntology .

      seas:ZigBeeCommunicationConnection a owl:Class ;
        rdfs:label "ZigBee Communication Connection"@en ;
        rdfs:comment """The class of ZigBee communication connections between communication devices."""@en ;
        rdfs:subClassOf seas:RadioCommunicationConnection ;
        rdfs:subClassOf [ owl:onProperty seas:connectsSystem ; owl:allValuesFrom  seas:ZigBeeCommunicationDevice ] ;
        rdfs:subClassOf [ owl:onProperty seas:connectsSystemAt ; owl:allValuesFrom  seas:ZigBeeCommunicationConnectionPoint ] ;
        vs:term_status "testing" ;
        rdfs:isDefinedBy seas:CommunicationOntology .

      seas:LoRaCommunicationConnection a owl:Class ;
        rdfs:label "LoRa Communication Connection"@en ;
        rdfs:comment """The class of LoRa communication connections between communication devices."""@en ;
        rdfs:subClassOf seas:RadioCommunicationConnection ;
        rdfs:subClassOf [ owl:onProperty seas:connectsSystem ; owl:allValuesFrom  seas:LoRaCommunicationDevice ] ;
        rdfs:subClassOf [ owl:onProperty seas:connectsSystemAt ; owl:allValuesFrom  seas:LoRaCommunicationConnectionPoint ] ;
        vs:term_status "testing" ;
        rdfs:isDefinedBy seas:CommunicationOntology .

      seas:BLECommunicationConnection a owl:Class ;
        rdfs:label "BLE Communication Connection"@en ;
        rdfs:comment """The class of BLE communication connections between communication devices."""@en ;
        rdfs:subClassOf seas:RadioCommunicationConnection ;
        rdfs:subClassOf [ owl:onProperty seas:connectsSystem ; owl:allValuesFrom  seas:BLECommunicationDevice ] ;
        rdfs:subClassOf [ owl:onProperty seas:connectsSystemAt ; owl:allValuesFrom  seas:BLECommunicationConnectionPoint ] ;
        vs:term_status "testing" ;
        rdfs:isDefinedBy seas:CommunicationOntology .

      seas:BluetoothCommunicationConnection a owl:Class ;
        rdfs:label "Bluetooth Communication Connection"@en ;
        rdfs:comment """The class of Bluetooth communication connections between communication devices."""@en ;
        rdfs:subClassOf seas:RadioCommunicationConnection ;
        rdfs:subClassOf [ owl:onProperty seas:connectsSystem ; owl:allValuesFrom  seas:BluetoothCommunicationDevice ] ;
        rdfs:subClassOf [ owl:onProperty seas:connectsSystemAt ; owl:allValuesFrom  seas:BluetoothCommunicationConnectionPoint ] ;
        vs:term_status "testing" ;
        rdfs:isDefinedBy seas:CommunicationOntology .

      seas:WiFiCommunicationConnection a owl:Class ;
        rdfs:label "WiFi Communication Connection"@en ;
        rdfs:comment """The class of WiFi communication connections between communication devices."""@en ;
        rdfs:subClassOf seas:RadioCommunicationConnection ;
        rdfs:subClassOf [ owl:onProperty seas:connectsSystem ; owl:allValuesFrom  seas:WiFiCommunicationDevice ] ;
        rdfs:subClassOf [ owl:onProperty seas:connectsSystemAt ; owl:allValuesFrom  seas:WiFiCommunicationConnectionPoint ] ;
        vs:term_status "testing" ;
        rdfs:isDefinedBy seas:CommunicationOntology .

      seas:EnOceanCommunicationConnection a owl:Class ;
        rdfs:label "EnOcean Communication Connection"@en ;
        rdfs:comment """The class of EnOcean communication connections between communication devices."""@en ;
        rdfs:subClassOf seas:RadioCommunicationConnection ;
        rdfs:subClassOf [ owl:onProperty seas:connectsSystem ; owl:allValuesFrom  seas:EnOceanCommunicationDevice ] ;
        rdfs:subClassOf [ owl:onProperty seas:connectsSystemAt ; owl:allValuesFrom  seas:EnOceanCommunicationConnectionPoint ] ;
        vs:term_status "testing" ;
        rdfs:isDefinedBy seas:CommunicationOntology .


## communication connection point

seas:CommunicationConnectionPoint a owl:Class ;
  rdfs:label "Communication Connection Point"@en ;
  rdfs:comment """The class of communication connection points of communication devices, at which they may be connected to other systems.
  For example, a water smart meter may have three communication connection points: Wireless M-Bus, Zigbee and LoRa:

```
  <waterSmartMeter> a seas:CommunicationDevice ;
    seas:connectsAt <waterSmartMeter_mbus> , <waterSmartMeter_zigbee> , <waterSmartMeter_lora> .
```
"""@en ;
  rdfs:subClassOf seas:ConnectionPoint ;
  rdfs:subClassOf [ owl:onProperty seas:connectionPointOf ; owl:allValuesFrom  seas:CommunicationDevice ] ;
  rdfs:subClassOf [ owl:onProperty seas:connectsSystemThrough ; owl:allValuesFrom  seas:CommunicationConnection ] ;
  vs:term_status "testing" ;
  rdfs:isDefinedBy seas:CommunicationOntology .

  seas:WireCommunicationConnectionPoint a owl:Class ;
    rdfs:label "Wire Communication Connection Point"@en ;
    rdfs:comment """The class of wire communication connection points between communication devices."""@en ;
    rdfs:subClassOf seas:CommunicationConnectionPoint ;
    rdfs:subClassOf [ owl:onProperty seas:connectionPointOf ; owl:allValuesFrom  seas:WireCommunicationDevice ] ;
    rdfs:subClassOf [ owl:onProperty seas:connectsSystemThrough ; owl:allValuesFrom  seas:WireCommunicationConnection ] ;
    vs:term_status "testing" ;
    rdfs:isDefinedBy seas:CommunicationOntology .
        
    seas:SerialCommunicationConnectionPoint a owl:Class ;
      rdfs:label "Serial Communication Connection Point"@en ;
      rdfs:comment """The class of Serial communication connection points between communication devices."""@en ;
      rdfs:subClassOf seas:WireCommunicationConnectionPoint ;
      rdfs:subClassOf [ owl:onProperty seas:connectionPointOf ; owl:allValuesFrom  seas:SerialCommunicationDevice ] ;
      rdfs:subClassOf [ owl:onProperty seas:connectsSystemThrough ; owl:allValuesFrom  seas:SerialCommunicationConnection ] ;
      vs:term_status "testing" ;
      rdfs:isDefinedBy seas:CommunicationOntology .
        
    seas:USBCommunicationConnectionPoint a owl:Class ;
      rdfs:label "USB Communication Connection Point"@en ;
      rdfs:comment """The class of USB communication connection points between communication devices."""@en ;
      rdfs:subClassOf seas:WireCommunicationConnectionPoint ;
      rdfs:subClassOf [ owl:onProperty seas:connectionPointOf ; owl:allValuesFrom  seas:USBCommunicationDevice ] ;
      rdfs:subClassOf [ owl:onProperty seas:connectsSystemThrough ; owl:allValuesFrom  seas:USBCommunicationConnection ] ;
      vs:term_status "testing" ;
      rdfs:isDefinedBy seas:CommunicationOntology .
       
  seas:WirelessCommunicationConnectionPoint a owl:Class ;
    rdfs:label "Wireless Communication Connection Point"@en ;
    rdfs:comment """The class of wireless communication connection points between communication devices."""@en ;
    rdfs:subClassOf seas:CommunicationConnectionPoint ;
    rdfs:subClassOf [ owl:onProperty seas:connectionPointOf ; owl:allValuesFrom  seas:WirelessCommunicationDevice ] ;
    rdfs:subClassOf [ owl:onProperty seas:connectsSystemThrough ; owl:allValuesFrom  seas:WirelessCommunicationConnection ] ;
    vs:term_status "testing" ;
    rdfs:isDefinedBy seas:CommunicationOntology .
         
    seas:RadioCommunicationConnectionPoint a owl:Class ;
      rdfs:label "Radio Communication Connection Point"@en ;
      rdfs:comment """The class of Radio communication connection points between communication devices."""@en ;
      rdfs:subClassOf seas:WirelessCommunicationConnectionPoint ;
      rdfs:subClassOf [ owl:onProperty seas:connectionPointOf ; owl:allValuesFrom  seas:RadioCommunicationDevice ] ;
      rdfs:subClassOf [ owl:onProperty seas:connectsSystemThrough ; owl:allValuesFrom  seas:RadioCommunicationConnection ] ;
      vs:term_status "testing" ;
      rdfs:isDefinedBy seas:CommunicationOntology .

      seas:SigFoxCommunicationConnectionPoint a owl:Class ;
        rdfs:label "SigFox Communication Connection Point"@en ;
        rdfs:comment """The class of SigFox communication connection points between communication devices."""@en ;
        rdfs:subClassOf seas:RadioCommunicationConnectionPoint ;
        rdfs:subClassOf [ owl:onProperty seas:connectionPointOf ; owl:allValuesFrom  seas:SigFoxCommunicationDevice ] ;
        rdfs:subClassOf [ owl:onProperty seas:connectsSystemThrough ; owl:allValuesFrom  seas:SigFoxCommunicationConnection ] ;
        vs:term_status "testing" ;
        rdfs:isDefinedBy seas:CommunicationOntology .

      seas:ZigBeeCommunicationConnectionPoint a owl:Class ;
        rdfs:label "ZigBee Communication Connection Point"@en ;
        rdfs:comment """The class of ZigBee communication connection points between communication devices."""@en ;
        rdfs:subClassOf seas:RadioCommunicationConnectionPoint ;
        rdfs:subClassOf [ owl:onProperty seas:connectionPointOf ; owl:allValuesFrom  seas:ZigBeeCommunicationDevice ] ;
        rdfs:subClassOf [ owl:onProperty seas:connectsSystemThrough ; owl:allValuesFrom  seas:ZigBeeCommunicationConnection ] ;
        vs:term_status "testing" ;
        rdfs:isDefinedBy seas:CommunicationOntology .

      seas:LoRaCommunicationConnectionPoint a owl:Class ;
        rdfs:label "LoRa Communication Connection Point"@en ;
        rdfs:comment """The class of LoRa communication connection points between communication devices."""@en ;
        rdfs:subClassOf seas:RadioCommunicationConnectionPoint ;
        rdfs:subClassOf [ owl:onProperty seas:connectionPointOf ; owl:allValuesFrom  seas:LoRaCommunicationDevice ] ;
        rdfs:subClassOf [ owl:onProperty seas:connectsSystemThrough ; owl:allValuesFrom  seas:LoRaCommunicationConnection ] ;
        vs:term_status "testing" ;
        rdfs:isDefinedBy seas:CommunicationOntology .
           
      seas:BLECommunicationConnectionPoint a owl:Class ;
        rdfs:label "BLE Communication Connection Point"@en ;
        rdfs:comment """The class of BLE communication connection points between communication devices."""@en ;
        rdfs:subClassOf seas:RadioCommunicationConnectionPoint ;
        rdfs:subClassOf [ owl:onProperty seas:connectionPointOf ; owl:allValuesFrom  seas:BLECommunicationDevice ] ;
        rdfs:subClassOf [ owl:onProperty seas:connectsSystemThrough ; owl:allValuesFrom  seas:BLECommunicationConnection ] ;
        vs:term_status "testing" ;
        rdfs:isDefinedBy seas:CommunicationOntology .
           
      seas:BluetoothCommunicationConnectionPoint a owl:Class ;
        rdfs:label "Bluetooth Communication Connection Point"@en ;
        rdfs:comment """The class of Bluetooth communication connection points between communication devices."""@en ;
        rdfs:subClassOf seas:RadioCommunicationConnectionPoint ;
        rdfs:subClassOf [ owl:onProperty seas:connectionPointOf ; owl:allValuesFrom  seas:BluetoothCommunicationDevice ] ;
        rdfs:subClassOf [ owl:onProperty seas:connectsSystemThrough ; owl:allValuesFrom  seas:BluetoothCommunicationConnection ] ;
        vs:term_status "testing" ;
        rdfs:isDefinedBy seas:CommunicationOntology .
           
      seas:WiFiCommunicationConnectionPoint a owl:Class ;
        rdfs:label "WiFi Communication Connection Point"@en ;
        rdfs:comment """The class of WiFi communication connection points between communication devices."""@en ;
        rdfs:subClassOf seas:RadioCommunicationConnectionPoint ;
        rdfs:subClassOf [ owl:onProperty seas:connectionPointOf ; owl:allValuesFrom  seas:WiFiCommunicationDevice ] ;
        rdfs:subClassOf [ owl:onProperty seas:connectsSystemThrough ; owl:allValuesFrom  seas:WiFiCommunicationConnection ] ;
        vs:term_status "testing" ;
        rdfs:isDefinedBy seas:CommunicationOntology .
            
      seas:EnOceanCommunicationConnectionPoint a owl:Class ;
        rdfs:label "EnOcean Communication Connection Point"@en ;
        rdfs:comment """The class of EnOcean communication connection points between communication devices."""@en ;
        rdfs:subClassOf seas:RadioCommunicationConnectionPoint ;
        rdfs:subClassOf [ owl:onProperty seas:connectionPointOf ; owl:allValuesFrom  seas:EnOceanCommunicationDevice ] ;
        rdfs:subClassOf [ owl:onProperty seas:connectsSystemThrough ; owl:allValuesFrom  seas:EnOceanCommunicationConnection ] ;
        vs:term_status "testing" ;
        rdfs:isDefinedBy seas:CommunicationOntology .
