# Copyright 2016 ITEA 12004 SEAS Project.
# 
# Licensed under the Apache License, Version 2.0 (the "License");
# you may not use this file except in compliance with the License.
# You may obtain a copy of the License at
# 
#      http://www.apache.org/licenses/LICENSE-2.0
# 
# Unless required by applicable law or agreed to in writing,
# distributed under the License is distributed on an "AS IS" BASIS,
# WITHOUT WARRANTIES OR CONDITIONS OF ANY KIND, either express or implied.
# See the License for the specific language governing permissions and
# limitations under the License.

@prefix rdf: <http://www.w3.org/1999/02/22-rdf-syntax-ns#> .
@prefix owl: <http://www.w3.org/2002/07/owl#> .
@prefix rdfs: <http://www.w3.org/2000/01/rdf-schema#> .
@prefix xsd: <http://www.w3.org/2001/XMLSchema#> .
@prefix dcterms: <http://purl.org/dc/terms/> .  
@prefix vann: <http://purl.org/vocab/vann/> .
@prefix voaf: <http://purl.org/vocommons/voaf#> .
@prefix vs: <http://www.w3.org/2003/06/sw-vocab-status/ns#> .
@prefix foaf: <http://xmlns.com/foaf/0.1/>.
@prefix ssn: <https://www.w3.org/ns/ssn/>.
@prefix dul: <http://www.ontologydesignpatterns.org/ont/dul/DUL.owl#>.
@prefix liner: <https://w3id.org/liner/>.
@prefix skos: <http://www.w3.org/2004/02/skos/core#>.
@prefix qb: <http://purl.org/linked-data/cube#>.
@prefix cdt: <http://w3id.org/lindt/custom_datatypes#>.

@prefix seas: <https://w3id.org/seas/>.
@base <https://w3id.org/seas/>.

voaf:Vocabulary a owl:Class .
dcterms:title a owl:AnnotationProperty .
dcterms:description a owl:AnnotationProperty .
dcterms:issued a owl:AnnotationProperty .
dcterms:modified a owl:AnnotationProperty .
dcterms:creator a owl:AnnotationProperty .
dcterms:contributor a owl:AnnotationProperty .
dcterms:license a owl:AnnotationProperty .
vann:preferredNamespacePrefix a owl:AnnotationProperty .
vann:preferredNamespaceUri a owl:AnnotationProperty .
vs:term_status a owl:AnnotationProperty .
foaf:Person a owl:Class .
foaf:name a owl:DatatypeProperty .



seas:ElectricLightSourceOntology a owl:Ontology , voaf:Vocabulary ;
  dcterms:title "The SEAS Electric Light Source Ontology."@en ;
  dcterms:description """The SEAS Electric Light source ontology describes Electric light sources.
  The figure below shows an overview of the electric light source taxonomy.
   [![LightsourceTaxonomy](https://w3id.org/seas/ElectricLightSourceTaxonomy-1.png)](https://w3id.org/seas/ElectricLightSourceTaxonomy-1.png)"""@en ;
  dcterms:issued "2017-02-22"^^xsd:date ;
  dcterms:modified "2017-08-23"^^xsd:date ;
  dcterms:creator [  a foaf:Person; foaf:name "Lynda TEMAL"] ;
  dcterms:contributor <http://www.maxime-lefrancois.info/me#> ;
  dcterms:license <https://www.apache.org/licenses/LICENSE-2.0> ;
  vann:preferredNamespacePrefix "seas" ;
  vann:preferredNamespaceUri <https://w3id.org/seas/> ;  
  owl:imports seas:ZoneLightingOntology , seas:ElectricPowerSystemOntology, seas:DeviceOntology ;
  owl:versionIRI <https://w3id.org/seas/ElectricLightSourceOntology-1.0> ;
  owl:versionInfo "v1.0" .


seas:ElectricLightSource a owl:Class ;
  rdfs:label "Electric Light Source"@en ;
  rdfs:comment """An electric light is a device that produces visible light by the flow of electric current. 
  It is the most common form of artificial lighting and is essential 
  to modern society, providing interior lighting for buildings and 
  exterior light for evening and nighttime activities. 
  In technical usage, a replaceable component that produces light from 
  electricity is called a lamp. (source: Wikipedia). 
  """@en ;
  rdfs:subClassOf seas:ElectricPowerSystem, seas:LightSource, seas:Device ;
  vs:term_status "testing" ;
  rdfs:isDefinedBy seas:ElectricLightSourceOntology .

seas:IncandescenceLight a owl:Class ;
  rdfs:subClassOf seas:ElectricLightSource;
  rdfs:label "Incandescence Light"@en ,
  "Lampe a Incandescence"@fr ;
  rdfs:comment """ Incandescence Light are Electric Light Source which produce light by a filament heated white-hot by electric current.
  (source: wikipedia)"""@en ;         
  vs:term_status "testing" ;
  rdfs:isDefinedBy seas:ElectricLightSourceOntology .

seas:IncandescentLamp a owl:Class ;
  rdfs:subClassOf seas:IncandescenceLight ;
  rdfs:comment """An incandescent light bulb, incandescent lamp or incandescent light globe 
  is an electric light with a wire filament heated to such a high temperature 
  that it glows with visible light (incandescence). 
  The filament, heated by passing an electric current through it, is protected from 
  oxidation with a glass or quartz bulb that is filled with inert gas or evacuated. 
  In a halogen lamp, filament evaporation is prevented by a chemical process that redeposits 
  metal vapor onto the filament, extending its life. The light bulb is supplied with 
  electric current by feed-through terminals or wires embedded in the glass. 
  Most bulbs are used in a socket which provides mechanical support and electrical connections.
  (source: wikipedia)"""@en ,
  """Le courant électrique passe dans le filament en tungstène et le porte à une 
  température élevée par effet Joule. Le filament devient incandescent : 
  il émet de la lumière ainsi que de la chaleur. Des atomes de tungstène sont éjectés 
  du filament par sublimation et sont déposés au niveau de la surface interne de l’ampoule 
  en verre plus froide. Il s’ensuit un noircissement de l’ampoule après un temps d’utilisation 
  relativement court. source: http://www.energieplus-lesite.be/index.php?id=10682"""@fr ;
  rdfs:label "Incandescent Lamp"@en , "Lampe Incandescente"@en ;
  vs:term_status "testing" ;
  rdfs:isDefinedBy seas:ElectricLightSourceOntology .



seas:HalogenLamp a owl:Class ;
  rdfs:subClassOf seas:IncandescenceLight ;
  rdfs:comment """A halogen lamp, also known as a tungsten halogen, quartz-halogen or quartz iodine lamp, 
  is an incandescent lamp that has a small amount of a halogen such as iodine 
  or bromine added. The combination of the halogen gas and the tungsten filament produces
  a halogen cycle chemical reaction which redeposits evaporated tungsten to the filament, 
  increasing its life and maintaining the clarity of the envelope. Because of this, a halogen lamp 
  can be operated at a higher temperature than a standard gas-filled lamp of similar power and
  operating life, producing light of a higher luminous efficacy and color temperature. 
  The small size of halogen lamps permits their use in compact optical systems for projectors and illumination. 
  (source: wikipedia)"""@en ,
  """La lampe halogène fonctionne sur le même principe qu’une lampe à incandescence : 
  elle produit de la lumière visible à partir d’un filament de tungstène porté à incandescence.
  Pour éviter une dégradation très rapide du filament, celui-ci est placé dans une ampoule à verre de quartz 
  (pour les hautes températures) renfermant des gaz halogénés à haute pression comme l’iode et 
  le brome. source : http://www.energieplus-lesite.be/index.php?id=10681"""@fr ;
  rdfs:label "Halogen Lamp"@en ,"Lampe Halogene"@fr ;
  vs:term_status "testing" ;
  rdfs:isDefinedBy seas:ElectricLightSourceOntology .

seas:LEDLamp a owl:Class ;
  rdfs:label "LED Lamp"@en ,"Lampe LED"@fr ;
  rdfs:subClassOf seas:ElectricLightSource ;
  rdfs:comment """An LED lamp is a light-emitting diode (LED) product which is 
  assembled into a lamp (or light bulb) for use in lighting fixtures. 
  LED lamps have a lifespan and electrical efficiency which are several times 
  greater than incandescent lamps, and are significantly more efficient than 
  most fluorescent lamps, with some chips able to emit more than 300 lumens per watt 
  (as claimed by Cree and some other LED manufacturers)."""@en ,
  """La lampe LED est un système complet conçu de manière à permettre le remplacement aisé des 
  technologies traditionnelles moins efficaces (retrofit). Ces lampes reprennent pour cela les formes
  et les culots normalisés des lampes traditionnelles. source: http://www.energieplus-lesite.be/index.php?id=17173"""@fr ;
  vs:term_status "testing" ;
  rdfs:isDefinedBy seas:ElectricLightSourceOntology .

seas:GasDischargeLamp a owl:Class ;
  rdfs:label "Gas Discharge Lamp"@en ;
  rdfs:subClassOf seas:ElectricLightSource;
  rdfs:comment """Gas-discharge lamps are a family of artificial light sources that generate light 
  by sending an electrical discharge through an ionized gas, a plasma. 
  Typically, such lamps use a noble gas (argon, neon, krypton, and xenon) or 
  a mixture of these gases. Some include additional substances, 
  like mercury, sodium, and metal halides, which are vaporized during startup to become 
  part of the gas mixture. (source:wikipedia)"""@en ,
  """Une lampe dite \"à décharge\" fonctionne par décharge d'un courant électrique dans une atmosphère gazeuse. 
  La décharge se fait au travers d'un tube à décharge qui se trouve lui-même dans une ampoule vide.
  Lorsqu'on met la lampe sous tension, des électrons sont émis par les deux électrodes de tungstène. 
  Lors de leur trajet au travers du tube à décharge, ils entrent en collision avec les atomes de gaz. 
  Il en résulte une libération d'énergie soit sous forme de lumière visible, 
  soit sous forme de rayonnement ultraviolet invisible (principalement pour les lampes 
  au mercure haute pression). Ce dernier est absorbé par le revêtement fluorescent présent 
  sur la face interne de la lampe et converti en rayonnement visible.
  Selon la pression du gaz dans le tube ou l'ampoule, on distingue les lampes à basse et à haute pression. source : http://www.energieplus-lesite.be/index.php?id=10685"""@fr ,
  """Une lampe à décharge est une lampe électrique constituée d'un tube ou d'une ampoule en verre remplie de gaz ou de vapeur métallique, sous haute ou basse pression, au travers duquel on fait passer un courant électrique, il s'ensuit une conversion en photons donc de la lumière.
  La couleur de la lumière émise par luminescence, par ces lampes dépend du gaz utilisé :
  Le néon donne une couleur rouge.
  Le mercure s'approche du bleu tout en produisant une quantité d'ultraviolet importante.
  Le sodium rayonne dans le jaune. Souvent on le mélange avec du néon pour rendre la lumière orangée.
  Le xénon (récemment employé pour l'éclairage des automobiles) est le gaz qui permet de s'approcher le plus possible du blanc pur. source:https://fr.wikipedia.org/wiki/Lampe_%C3%A0_d%C3%A9charge"""@fr ;
  vs:term_status "testing" ;
  rdfs:isDefinedBy seas:ElectricLightSourceOntology .

seas:LowPressureDischargeLamp a owl:Class ;
  rdfs:subClassOf seas:GasDischargeLamp ;
  rdfs:label "Low Pressure Discharge Lamp"@en ;
  rdfs:comment """Low-pressure lamps have working pressure much less than atmospheric pressure. 
  For example, common fluorescent lamps operate at a pressure of about 0.3% of 
  atmospheric pressure. (source: wikipedia)"""@en ;
  vs:term_status "testing" ;
  rdfs:isDefinedBy seas:ElectricLightSourceOntology .

seas:HighPressureDischargeLamp a owl:Class ;
  rdfs:subClassOf seas:GasDischargeLamp ;
  rdfs:label "High Pressure Discharge Lamp"@en;
  rdfs:comment """High-pressure lamps have a discharge that takes place in gas under slightly 
  less to greater than atmospheric pressure. For example, a high pressure sodium 
  lamp has an arc tube under 100 to 200 torr pressure, about 14% to 28% of atmospheric 
  pressure; some automotive HID headlamps have up to 50 bar or fifty times atmospheric 
  pressure. (source:wikipedia)"""@en ;
  vs:term_status "testing" ;
  rdfs:isDefinedBy seas:ElectricLightSourceOntology .

seas:HighPressureMercuryLamp a owl:Class ;
  rdfs:subClassOf seas:HighPressureDischargeLamp ;
  rdfs:label "High Pressure Mercury Lamp"@en ,
  "Lampe Mercure Haute Pression"@fr;
  rdfs:comment """L'ampoule contient de la vapeur de mercure et de l'argon.
  La lumière est émise exclusivement sous forme de rayons 
  ultraviolets invisibles rendus visibles par les poudres 
  fluorescentes placées sur la face interne de l'ampoule.
  La lampe à mercure haute pression dispose d'électrodes 
  auxiliaires servant de démarreur interne. Pour bien fonctionner, 
  elle ne doit donc être équipée que d'un ballast et d'un condensateur. 
  source :http://www.energieplus-lesite.be/index.php?id=10686"""@fr,
  """A High pressure mercury-vapor lamp is a  high pressure gas discharge 
  lamp that uses an electric arc through vaporized mercury under high pression
  to produce light. (source:wikipedia)"""@en ;
  vs:term_status "testing" ;
  rdfs:isDefinedBy seas:ElectricLightSourceOntology .

seas:LowPressureMercuryLamp a owl:Class ;
  rdfs:subClassOf seas:LowPressureDischargeLamp ;
  rdfs:label "Low Pressure Mercury Lamp"@en ,
  "Lampe Mercure Basse Pression"@fr;
  rdfs:comment """L'ampoule contient de la vapeur de mercure et de l'argon.
  La lumière est émise exclusivement sous forme de rayons 
  ultraviolets invisibles rendus visibles par les poudres 
  fluorescentes placées sur la face interne de l'ampoule.
  source :http://www.energieplus-lesite.be/index.php?id=10686"""@fr,
  """A Low pressure mercury-vapor lamp is a low pressure gas discharge 
  lamp that uses an electric arc through vaporized mercury under low pression
  to produce light. (source:wikipedia)"""@en ;
  vs:term_status "testing" ;
  rdfs:isDefinedBy seas:ElectricLightSourceOntology .     


seas:HighPressureSodiumLamp a owl:Class ;
  rdfs:subClassOf seas:HighPressureDischargeLamp ;
  rdfs:label "High Pressure Sodium Lamp"@en ,
  "Lampe Sodium Basse Pression"@fr;
  rdfs:comment """High-pressure sodium lamps are high pressur gas discharge lamp which produce a broader spectrum of 
  light than the low-pressure lamps, but they still have poorer color rendering than 
  other types of lamps. Low-pressure sodium lamps only give monochromatic yellow light 
  and so inhibit color vision at night. They have been widely used in industrial lighting, 
  especially in large manufacturing facilities, and are commonly used as plant grow lights. 
  They have also been widely used for outdoor area lighting, such as on roadways, parking lots 
  and security areas. (source: wikipedia)"""@en ,
  """La lampe à vapeur de sodium fait partie des lampes à décharge. Son principe de fonctionnement est donc identique."""@fr;
  vs:term_status "testing" ;
  rdfs:isDefinedBy seas:ElectricLightSourceOntology .

seas:LowPressureSodiumLamp a owl:Class ;
  rdfs:label  "Low Pressure Sodium Lamp"@en,
  "Lampe Sodium Basse Pression"@fr ,
  "SBP"@fr ;
  rdfs:subClassOf seas:LowPressureDischargeLamp ;
  rdfs:comment """La lampe au sodium basse pression fait partie des lampes à décharge. 
  Son principe de fonctionnement est donc identique. L'ensemble amorceur, ballast conventionnel
  et condensateur peut être remplacé par un ballast électronique.
  Particularités: Cette lampe est constituée d'un tube à décharge en forme de \"U\" logé
  dans une ampoule extérieure. Le tube à décharge contient un mélange de vapeur de sodium 
  et de gaz tels que le néon et l'argon. La lumière est émise, en majeure partie sous forme de 
  rayonnements visibles, sa face interne n'est donc pas recouverte d'une couche de poudre fluorescente. source http://www.energieplus-lesite.be/index.php?id=10687"""@fr ,
  """Low-pressure sodium lamp is a gas-discharge lamp that uses sodium in an excited state to 
  produce light at a characteristic wavelength near 589 nm. They are highly efficient electrical light sources, 
  but their yellow light restricts applications to outdoor lighting such as street lamps. (source : wikipedia)"""@en ;
  vs:term_status "testing" ;
  rdfs:isDefinedBy seas:ElectricLightSourceOntology .

seas:MetalHalideLamp a owl:Class ;
  rdfs:subClassOf seas:HighPressureDischargeLamp ;
  rdfs:comment """A metal-halide lamp  is a  high-intensity discharge (HID) gas discharge 
  lamp which is an electrical lamp that produces light by an electric arc through
  a gaseous mixture of vaporized mercury and metal halides (compounds of metals 
  with bromine or iodine). It is a type of high-intensity discharge (HID) gas discharge
  lamp. (source:wikipedia)"""@en ;
  rdfs:label "Lampe halogenure metallique"@fr ,
  "Metal Halide Lamp"@en ;                          
  vs:term_status "testing" ;
  rdfs:isDefinedBy seas:ElectricLightSourceOntology .

seas:CeramicMetalHalideLamp a owl:Class ;
  rdfs:subClassOf seas:MetalHalideLamp ;
  rdfs:comment """The ceramic discharge metal-halide (CDM) lamp, often referred to as Ceramic Metal Halide lamp
  (CMH) is a source of light that is a type of metal-halide lamp which is 10-20% more efficient
  than the traditional quartz metal halide and produces a superior color rendition (80-96 CRI). 
  (source:wikipedia)"""@en ;
  rdfs:label "Ceramic Metal Halide Lamp"@en ;                          
  vs:term_status "testing" ;
  rdfs:isDefinedBy seas:ElectricLightSourceOntology .

seas:FluorescentTube a owl:Class ;
  rdfs:subClassOf seas:LowPressureMercuryLamp;
  rdfs:comment """A fluorescent lamp or a fluorescent tube is a low pressure mercury-vapor gas-discharge
  lamp that uses fluorescence to produce visible light. An electric current in the gas 
  excites mercury vapor which produces short-wave ultraviolet light that then causes 
  a phosphor coating on the inside of the lamp to glow. A fluorescent lamp converts electrical 
  energy into useful light much more efficiently than incandescent lamps. The typical luminous 
  efficacy of fluorescent lighting systems is 50–100 lumens per watt, several times the efficacy 
  of incandescent bulbs with comparable light output. (wikipedia:Source)"""@en ,
  """Les lampes fluorescentes font partie des lampes à décharge. Elles fonctionnent par décharge d'un 
  courant électrique dans une atmosphère gazeuse. Les lampes fluorescentes utilisent de la 
  vapeur de mercure sous basse pression. source :http://www.energieplus-lesite.be/index.php?id=10683"""@fr ;
  rdfs:label "Fluorescent Tube"@en ,
  "TF"@fr ,
  "Tube Fluorescent"@fr ;                    
  vs:term_status "testing" ;
  rdfs:isDefinedBy seas:ElectricLightSourceOntology .

seas:CompactFluorescentLamp a owl:Class ;
  rdfs:subClassOf seas:LowPressureMercuryLamp;
  rdfs:label "Compact Fluorescent Lamp"@en ,
  "FLC"@fr ,
  "Lampe Fluocompactes"@fr  ;
  rdfs:comment """A compact fluorescent lamp (CFL), also called compact fluorescent light, 
  energy-saving light, and compact fluorescent tube, is a fluorescent lamp designed 
  to replace an incandescent light bulb; some types fit into light fixtures designed 
  for incandescent bulbs. The lamps use a tube which is curved or folded to fit into 
  the space of an incandescent bulb, and a compact electronic ballast in the base of 
  the lamp. (source: wikipedia)"""@en;           
  vs:term_status "testing" ;
  rdfs:isDefinedBy seas:ElectricLightSourceOntology .

seas:InductionLamp a owl:Class ;
  rdfs:subClassOf seas:LowPressureMercuryLamp ;
  rdfs:comment """La lampe à induction est une lampe à mercure basse pression comme le tube fluorescent 
  et la lampe fluocompacte. Comme dans la lampe fluorescente, la lumière est produite par 
  ionisation des atomes de gaz présents dans l'ampoule. Les rayonnements invisibles produits 
  sont rendus visibles grâce à une poudre fluorescente présente sur la face interne de l'ampoule.
  Dans une lampe à induction, il n'y a pas d'électrode. L'ionisation des atomes est réalisée 
  par un champ électromagnétique créé par la circulation d'un courant à haute fréquence dans une 
  bobine appelée \"antenne\". Cette bobine est placée au centre de l'ampoule dans la cavité prévue 
  à cet effet. Le courant à haute fréquence est produit par un générateur extérieur. Celui-ci est 
  directement relié à l'antenne. source :http://www.energieplus-lesite.be/index.php?id=10680"""@fr,
  """Induction light is a gas discharge lamp in which the power required to generate light is transferred
  from outside the lamp envelope to the gas inside via an electric or magnetic field, in contrast with a 
  typical gas discharge lamp that uses internal electrodes connected to the power supply by conductors 
  that pass through the lamp envelope (source:wikipedia)"""@en ;
  rdfs:label "Induction Lamp"@en ,
  "Lampe à Induction"@fr ;
  vs:term_status "testing" ;
  rdfs:isDefinedBy seas:ElectricLightSourceOntology .


#######################################
#Color Temperature
#######################################
seas:ColorTemperatureProperty a owl:Class ;
  rdfs:label "Color Temperature Property"@en ;
  rdfs:comment """The color temperature of a light source is the temperature of an ideal black-body radiator that radiates light of a color comparable 
                  to that of the light source. Color temperature is a characteristic of visible light that has important applications in lighting, photography, 
                  videography, publishing, manufacturing, astrophysics, horticulture, and other fields.(source:wikipedia)"""@en,
                  "Correlated color temperature of the lamp"@en ;
  rdfs:subClassOf seas:Property ;
  vs:term_status "testing" ;
  rdfs:isDefinedBy seas:ElectricLightSourceOntology .

seas:ColorTemperatureEvaluation a owl:Class ;
  rdfs:label "Color Temperature Evaluation"@en ;
  rdfs:comment """The class of evaluation for color temperature properties"""@en ;
  rdfs:subClassOf seas:Evaluation ;
  rdfs:subClassOf [ owl:onProperty seas:evaluationOf ; owl:someValuesFrom seas:ColorTemperatureProperty ] ;
  owl:equivalentClass [ owl:onProperty seas:evaluationOf ; owl:someValuesFrom seas:ColorTemperatureProperty ] ;
  vs:term_status "testing" ;
  rdfs:isDefinedBy seas:ElectricLightSourceOntology.

seas:colorTemperature a owl:ObjectProperty , owl:FunctionalProperty ;
  rdfs:label "colorTemperature"@en ;
  rdfs:comment """The color temperature of some light source."""@en ;
  rdfs:subPropertyOf seas:hasProperty ;
  rdfs:domain seas:LightSource ;
  rdfs:range seas:ColorTemperatureProperty ;
  vs:term_status "testing" ;
  rdfs:isDefinedBy seas:ElectricLightSourceOntology .


#######################################
#Color Rendering Index
#######################################
seas:ColorRenderingIndexProperty a owl:Class ;
  rdfs:label "Color Rendering Index Property"@en ;
  rdfs:comment """A color rendering index (CRI) is a quantitative measure of the ability of a light source to reveal the colors of various objects faithfully 
                  in comparison with an ideal or natural light source. (source:wikipedia)"""@en ;
  rdfs:subClassOf seas:Property ;
  vs:term_status "testing" ;
  rdfs:isDefinedBy seas:ElectricLightSourceOntology .

seas:ColorRenderingIndexEvaluation a owl:Class ;
  rdfs:label "Color Rendering Index Evaluation"@en ;
  rdfs:comment """The class of evaluation for color rendering index properties"""@en ;
  rdfs:subClassOf seas:Evaluation ;
  rdfs:subClassOf [ owl:onProperty seas:evaluationOf ; owl:someValuesFrom seas:ColorRenderingIndexProperty ] ;
  owl:equivalentClass [ owl:onProperty seas:evaluationOf ; owl:someValuesFrom seas:ColorRenderingIndexProperty ] ;
  vs:term_status "testing" ;
  rdfs:isDefinedBy seas:ElectricLightSourceOntology.

seas:colorRenderingIndex a owl:ObjectProperty , owl:FunctionalProperty ;
  rdfs:label "color rendering index"@en ;
  rdfs:comment """The color rendering index of some light source."""@en ;
  rdfs:subPropertyOf seas:hasProperty ;
  rdfs:domain seas:LightSource ;
  rdfs:range seas:ColorRenderingIndexProperty ;
  vs:term_status "testing" ;
  rdfs:isDefinedBy seas:ElectricLightSourceOntology .


#######################################
#Luminouce Flux
#######################################

seas:LuminousFluxProperty a owl:Class ;
  rdfs:label "Luminous Flux Property"@en ;
  rdfs:comment """In photometry, luminous flux or luminous power is the measure of the perceived power of light.(source:wikipedia)"""@en,
                "Maximum light output which can be provided by the lamp. source (http://fiware-datamodels.readthedocs.io/en/latest/StreetLighting/StreetlightModel/doc/spec/index.html)" ;
  rdfs:subClassOf seas:Property ;
  vs:term_status "testing" ;
  rdfs:isDefinedBy seas:ElectricLightSourceOntology .

seas:LuminousFluxEvaluation a owl:Class ;
  rdfs:label "Luminous Flux Evaluation"@en ;
  rdfs:comment """The class of evaluation for Luminous Flux properties"""@en ;
  rdfs:subClassOf seas:Evaluation ;
  rdfs:subClassOf [ owl:onProperty seas:evaluationOf ; owl:someValuesFrom seas:LuminousFluxProperty ] ;
  owl:equivalentClass [ owl:onProperty seas:evaluationOf ; owl:someValuesFrom seas:LuminousFluxProperty ] ;
  vs:term_status "testing" ;
  rdfs:isDefinedBy seas:ElectricLightSourceOntology.

seas:luminousFlux a owl:ObjectProperty , owl:FunctionalProperty ;
  rdfs:label "luminous flux"@en ;
  rdfs:comment """The luminous flux of some light source."""@en ;
  rdfs:subPropertyOf seas:hasProperty ;
  rdfs:domain seas:LightSource ;
  rdfs:range seas:LuminousFluxProperty ;
  vs:term_status "testing" ;
  rdfs:isDefinedBy seas:ElectricLightSourceOntology .



#######################################
#Luminouce Energy
#######################################
seas:LuminousEnergyProperty a owl:Class ;
  rdfs:label "Luminous Energy Property"@en ;
  rdfs:comment """In photometry, luminous energy is the perceived energy of light. This is sometimes called the quantity of light.(source:wikipedia)"""@en;
  rdfs:subClassOf seas:Property ;
  vs:term_status "testing" ;
  rdfs:isDefinedBy seas:ElectricLightSourceOntology .

seas:LuminousEnergyEvaluation a owl:Class ;
  rdfs:label "Luminous Energy Evaluation"@en ;
  rdfs:comment """The class of evaluation for Luminous Energy properties"""@en ;
  rdfs:subClassOf seas:Evaluation ;
  rdfs:subClassOf [ owl:onProperty seas:evaluationOf ; owl:someValuesFrom seas:LuminousEnergyProperty ] ;
  owl:equivalentClass [ owl:onProperty seas:evaluationOf ; owl:someValuesFrom seas:LuminousEnergyProperty ] ;
  vs:term_status "testing" ;
  rdfs:isDefinedBy seas:ElectricLightSourceOntology.

seas:luminousEnergy a owl:ObjectProperty , owl:FunctionalProperty ;
  rdfs:label "luminous energy"@en ;
  rdfs:comment """The luminous energy of some light."""@en ;
  rdfs:subPropertyOf seas:hasProperty ;
  rdfs:domain seas:LightSource ;
  rdfs:range seas:LuminousEnergyProperty ;
  vs:term_status "testing" ;
  rdfs:isDefinedBy seas:ElectricLightSourceOntology .



#######################################
#Luminouce Intensity
#######################################
seas:LuminousIntensityProperty a owl:Class ;
  rdfs:label "Luminous Intensity Property"@en ;
  rdfs:comment """In photometry, luminous intensity is a measure of the wavelength-weighted power emitted by a light source in a particular direction 
  per unit solid angle, based on the luminosity function, a standardized model of the sensitivity of the human eye. The SI unit of luminous intensity 
  is the candela (cd), an SI base unit.(source:wikipedia)"""@en;
  rdfs:subClassOf seas:Property ;
  vs:term_status "testing" ;
  rdfs:isDefinedBy seas:ElectricLightSourceOntology .

seas:LuminousIntensityEvaluation a owl:Class ;
  rdfs:label "Luminous Flux Evaluation"@en ;
  rdfs:comment """The class of evaluation for Luminous Intensity properties"""@en ;
  rdfs:subClassOf seas:Evaluation ;
  rdfs:subClassOf [ owl:onProperty seas:evaluationOf ; owl:someValuesFrom seas:LuminousIntensityProperty ] ;
  owl:equivalentClass [ owl:onProperty seas:evaluationOf ; owl:someValuesFrom seas:LuminousIntensityProperty ] ;
  vs:term_status "testing" ;
  rdfs:isDefinedBy seas:ElectricLightSourceOntology.

seas:luminousIntensity a owl:ObjectProperty , owl:FunctionalProperty ;
  rdfs:label "luminous intensity"@en ;
  rdfs:comment """The luminous intensity of some light."""@en ;
  rdfs:subPropertyOf seas:hasProperty ;
  rdfs:domain seas:LightSource ;
  rdfs:range seas:LuminousIntensityProperty ;
  vs:term_status "testing" ;
  rdfs:isDefinedBy seas:ElectricLightSourceOntology .

#######################################
#Luminouce Efficacy
#######################################

seas:LuminousEfficacyProperty a owl:Class ;
  rdfs:label "Luminous Efficacy Property"@en ;
  rdfs:comment """Luminous efficacy is a measure of how well a light source produces visible light. It is the ratio of luminous flux to power, 
                  measured in lumens per watt in SI.(source:wikipedia)"""@en;
  rdfs:subClassOf seas:Property ;
  vs:term_status "testing" ;
  rdfs:isDefinedBy seas:ElectricLightSourceOntology .

seas:LuminousEfficacyEvaluation a owl:Class ;
  rdfs:label "Luminous Efficacy Evaluation"@en ;
  rdfs:comment """The class of evaluation for Luminous Efficacy properties"""@en ;
  rdfs:subClassOf seas:Evaluation ;
  rdfs:subClassOf [ owl:onProperty seas:evaluationOf ; owl:someValuesFrom seas:LuminousEfficacyProperty ] ;
  owl:equivalentClass [ owl:onProperty seas:evaluationOf ; owl:someValuesFrom seas:LuminousEfficacyProperty ] ;
  vs:term_status "testing" ;
  rdfs:isDefinedBy seas:ElectricLightSourceOntology.

seas:luminousEfficacy a owl:ObjectProperty , owl:FunctionalProperty ;
  rdfs:label "luminous efficacy"@en ;
  rdfs:comment """The luminous efficacy of some light source."""@en ;
  rdfs:subPropertyOf seas:hasProperty ;
  rdfs:domain seas:LightSource ;
  rdfs:range seas:LuminousEfficacyProperty ;
  vs:term_status "testing" ;
  rdfs:isDefinedBy seas:ElectricLightSourceOntology .

#######################################
# illuminance
#######################################
seas:IlluminanceProperty a owl:Class ; 
      rdfs:label "Illuminance Property"@en ;
      rdfs:comment """Illuminance is the total luminous flux incident on a surface, per unit area. It is a measure of how much the incident light 
      illuminates the surface, wavelength-weighted by the luminosity function to correlate with human brightness perception. 
      An Illuminance Property is a property which is inherent in a lightsource."""@en ;
      rdfs:subClassOf seas:Property;
      vs:term_status "testing" ;
      rdfs:isDefinedBy seas:StreetLightSystemOntology .

seas:IlluminanceEvaluation  a owl:Class ; 
      rdfs:label "Illuminance Evaluation"@en ;
      rdfs:comment """A Illuminance Evaluation is an evaluation of Illuminance Property."""@en ;
      rdfs:subClassOf seas:Evaluation;
      vs:term_status "testing" ;
      rdfs:isDefinedBy seas:StreetLightSystemOntology .

seas:illuminance a owl:ObjectProperty, owl:FunctionalProperty;
      rdfs:label "illuminance"@en ;
      rdfs:comment """The illuminance is a property of some physical entity."""@en ;
      rdfs:subPropertyOf seas:hasProperty ;
      rdfs:domain seas:FeatureOfInterest ;
      rdfs:range seas:LightActuator ;
      vs:term_status "testing" ;
      rdfs:isDefinedBy seas:StreetLightSystemOntology .

