# Copyright 2016 ITEA 12004 SEAS Project.
#
# Licensed under the Apache License, Version 2.0 (the "License");
# you may not use this file except in compliance with the License.
# You may obtain a copy of the License at
#
#      http://www.apache.org/licenses/LICENSE-2.0
#
# Unless required by applicable law or agreed to in writing,
# distributed under the License is distributed on an "AS IS" BASIS,
# WITHOUT WARRANTIES OR CONDITIONS OF ANY KIND, either express or implied.
# See the License for the specific language governing permissions and
# limitations under the License.

@prefix rdf: <http://www.w3.org/1999/02/22-rdf-syntax-ns#> .
@prefix owl: <http://www.w3.org/2002/07/owl#> .
@prefix rdfs: <http://www.w3.org/2000/01/rdf-schema#> .
@prefix xsd: <http://www.w3.org/2001/XMLSchema#> .
@prefix dc: <http://purl.org/dc/terms/> .
@prefix vann: <http://purl.org/vocab/vann/> .
@prefix voaf: <http://purl.org/vocommons/voaf#> .
@prefix vs: <http://www.w3.org/2003/06/sw-vocab-status/ns#> .
@prefix saref: <https://w3id.org/saref#>.
@prefix cc: <http://creativecommons.org/ns#>.
@prefix foaf: <http://xmlns.com/foaf/0.1/>.
@prefix pep: <https://w3id.org/pep/> .
@prefix gr: <http://purl.org/goodrelations/v1#>.
@prefix skos: <http://www.w3.org/2004/02/skos/core#>.
@prefix dbr: <http://dbpedia.org/resource/> .

@prefix seas: <https://w3id.org/seas/>.
@base <https://w3id.org/seas/>.

voaf:Vocabulary a owl:Class .
dc:title a owl:AnnotationProperty .
dc:description a owl:AnnotationProperty .
dc:issued a owl:AnnotationProperty .
dc:modified a owl:AnnotationProperty .
dc:creator a owl:AnnotationProperty .
dc:contributor a owl:AnnotationProperty .
cc:license a owl:AnnotationProperty .
vann:preferredNamespacePrefix a owl:AnnotationProperty .
vann:preferredNamespaceUri a owl:AnnotationProperty .
vs:term_status a owl:AnnotationProperty .
foaf:Person a owl:Class .
foaf:name a owl:DatatypeProperty .



seas:SmartMeterOntology rdf:type voaf:Vocabulary , owl:Ontology ;
  dc:title "The SEAS Smart Meter ontology"@en ;
  dc:description """The SEAS Smart Meter ontology defines `seas:SmartMeter` as physical system (`seas:Sensor`) that are designed to Compute 
  Metering on different  amount of matter, such as natural gas, Water and Electricity. Smart Meters are connected systems 
  which are able to send metering evalutation to some managing systems. In the current version Smart meter are composed 
  (`seas:subsystemOf`) of a traditional meter and a connector module which is connected to the meter. 
  The two systems forme the smartMeter.
  In this ontology you will find concepts about 
    - Meters (`seas:WaterMeter`, `seas:GasMeter`, `seas:ElectricityMeter`) and thier metering mechanism (`seas:Pulse`, `seas:Optic`, `seas:Disc`..). 
    - Connectors module (we treat currently the case of fludia connectors seas:FludiaConnectors), these connectors can communicate thanks to  a 
    - `seas:CommunicationProtocol` such as `seas:LoraProtocol` and `seas:SigFoxProtocol`. These protocoles communicate through `seas:RadioWaves` Technologies.  
"""@en ;
  dc:issued "2016-05-10"^^xsd:date ;
  dc:modified "2016-11-24"^^xsd:date ;
  dc:creator [  a foaf:Person; foaf:name "Lynda TEMAL"] ;
  dc:contributor <http://www.maxime-lefrancois.info/me#> ;
  cc:license <https://www.apache.org/licenses/LICENSE-2.0> ;
  vann:preferredNamespacePrefix "seas" ;
  vann:preferredNamespaceUri <https://w3id.org/seas/> ;
  owl:imports seas:DeviceOntology, seas:ElectricPowerSystemOntology ;
  owl:versionIRI <https://w3id.org/seas/SmartMeterOntology-1.0> ;
  owl:versionInfo "v1.0" .


## Concept added to model  information about the USE case
seas:Meter a owl:Class;
          rdfs:subClassOf seas:Sensor;
          rdfs:label "Meter"@en;
          skos:altLabel "Measuring instrument"@en;
          rdfs:comment "A Meter is a sensor that is designed to allow to carry out a metering process"@en;
          rdfs:subClassOf [ owl:onProperty pep:implements ; owl:someValuesFrom seas:Metering ] ;
          owl:equivalentClass [ owl:onProperty pep:implements ; owl:someValuesFrom seas:Metering ] ;
          vs:term_status "testing" ;
          rdfs:isDefinedBy seas:SmartMeterOntology .


seas:Metering a owl:Class;
              rdfs:label "Metering"@en ;
              rdfs:comment """Metering is the process that allow to carry out some measuring on a property."""@en ;
              rdfs:subClassOf seas:Sensing ;
              vs:term_status "testing" ;
              rdfs:isDefinedBy seas:SmartMeterOntology .


seas:MeteringExecution a owl:Class ;
  rdfs:label "Metering Execution"@en ;
  rdfs:comment """An MeteringExecution is the execution of the measuring process which is executed by a meter device."""@en ;
  rdfs:subClassOf seas:Observation ;
  rdfs:subClassOf [ owl:onProperty pep:executedBy ; owl:someValuesFrom seas:Meter ] ;
  rdfs:subClassOf [ owl:onProperty pep:methodUsed ; owl:someValuesFrom seas:Metering ] ;
  rdfs:subClassOf [ owl:onProperty seas:observesProperty ; owl:someValuesFrom seas:Property ] ;
  owl:equivalentClass [ owl:onProperty pep:methodUsed ; owl:someValuesFrom seas:Metering ] ;
  vs:term_status "testing" ;
  rdfs:isDefinedBy seas:SmartMeterOntology .



seas:measuresProperty a owl:ObjectProperty ;
  rdfs:subPropertyOf seas:observesProperty;
  rdfs:label "measures property"@en ;
  rdfs:comment """Links a Metering, meter, or metering execution, to a property it measures.

If a Metering measures a property, then any meter that implements this Metering also measures this property, and any MeteringExecution that used this Metering also measures this property. 
Furthermore, if a meter measures a property, then any metering execution executed by this meter also measures this property:

```
seas:measuresProperty < pep:implements o seas:measuresProperty .
seas:measuresProperty < pep:methodUsed o seas:measuresProperty .
seas:measuresProperty < pep:executedBy o seas:measuresProperty .
```
"""@en ;
  rdfs:domain [ owl:unionOf ( seas:Metering seas:Meter seas:MeteringExecution ) ] ;
  rdfs:range seas:Property ;
  owl:propertyChainAxiom ( pep:implements seas:measuresProperty ) ;
  owl:propertyChainAxiom ( pep:methodUsed seas:measuresProperty ) ;
  owl:propertyChainAxiom ( pep:executedBy seas:measuresProperty ) ;
  vs:term_status "testing" ;
  rdfs:isDefinedBy seas:SmartMeterOntology .


seas:measures a owl:ObjectProperty ;
  rdfs:subPropertyOf seas:observes;
  rdfs:label "measures"@en ;
  rdfs:comment """Links a metering, meter, or metering execution, to the feature of interest a property of which it measures.

If `x` measures a property, then it also measures the feature of interest of this property:

```
seas:measures < seas:measuresProperty o seas:isPropertyOf .
```

If a metering measures a feature of interest, then any meter that implements this metering also measures this feature of interest, and any metering execution that used this metering also measures this feature of interest. 
Furthermore, if a meter measures a feature of interest, then any Metering Execution executed by this meter also measures this feature of interest:

```
seas:measures < pep:methodUsed o seas:measures .
seas:measures < pep:methodUsed o seas:measures .
seas:measures < pep:executedBy o seas:measures .
```
  
"""@en ;
  rdfs:domain [ owl:unionOf ( seas:Metering seas:Meter seas:MeteringExecution ) ] ;
  rdfs:range seas:FeatureOfInterest ;
#  owl:propertyChainAxiom ( seas:observesProperty seas:isPropertyOf ) ; # not allowed in OWL 2 DL
  owl:propertyChainAxiom ( pep:implements seas:measures ) ;
  owl:propertyChainAxiom ( pep:methodUsed seas:measures ) ;
  owl:propertyChainAxiom ( pep:executedBy seas:measures ) ;
  vs:term_status "testing" ;
  rdfs:isDefinedBy seas:SmartMeterOntology .


seas:ConnectorModule a owl:Class; # the part which is connected to a meter to send the consumption data 
                rdfs:subClassOf seas:Sensor;
                rdfs:label "Connector Module"@en;
                rdfs:comment "A connector Module is a sensor which is designed to be connected to a meter. It can read the metering data (with some methods) and send the data at regular frequency to a configured  system."@en;
                vs:term_status "testing" ;
                rdfs:isDefinedBy seas:SmartMeterOntology .


seas:WaterMeter  a owl:Class ;
                rdfs:comment """A water meter is a Meter which is designed to be able to measure the quantity of water that flow through a pipe. 
                                The waterMeter can measure water consumption or water supplying. 
                                Every `seas:WaterMeter` use a metering mechanism (`seas:MeteringMechanism` such as `seas:Pulse` , `seas:Disc`) which 
                                allow them to measure the volume of water (`seas:WaterVolume`) that flow in the pipe."""^^xsd:string ;
                rdfs:label "Water Meter"^^xsd:string ;
                rdfs:subClassOf seas:Meter ;
                rdfs:subClassOf [ owl:onProperty seas:measuresProperty ; owl:someValuesFrom seas:WaterVolumeProperty ] ;
                rdfs:subClassOf [ owl:onProperty seas:hasMeteringMechanism ; owl:maxQualifiedCardinality "1"^^xsd:nonNegativeInteger; owl:hasValue seas:MeteringMechanism] ;
                vs:term_status "testing"^^xsd:string ;
                rdfs:isDefinedBy seas:SmartMeterOntology . 

seas:DisplacementWaterMeter  a owl:Class ;
                rdfs:comment """This type of water meter is most often used in residential and small commercial applications and 
                                homes. Displacement meters are commonly referred to as Positive Displacement, or "PD" meters. 
                                Two common types are oscillating piston meters and nutating disk meters. Either method relies on 
                                the water to physically displace the moving measuring element in direct proportion to the amount 
                                of water that passes through the meter. The piston or disk moves a magnet that drives the register."""^^xsd:string ;
                rdfs:label "Displacement Water Meter"^^xsd:string ;
                rdfs:subClassOf seas:WaterMeter ;
                vs:term_status "testing"^^xsd:string ;
                rdfs:isDefinedBy seas:SmartMeterOntology .

seas:VelocityWaterMeter  a owl:Class ;
                rdfs:comment """A velocity-type water meter measures the velocity of flow through a meter of a known internal capacity.
                             The speed of the flow can then be converted into volume of flow to determine the usage. 
                             There are several types of meters that measure water flow velocity, including jet meters (single-jet and multi-jet), 
                             turbine meters, propeller meters and mag meters. Most velocity-based meters have an adjustment vane for calibrating 
                             the meter to the required accuracy."""^^xsd:string ;
                rdfs:label "Velocity Water Meter"^^xsd:string ;
                rdfs:subClassOf seas:WaterMeter ;
                vs:term_status "testing"^^xsd:string ;
                rdfs:isDefinedBy seas:SmartMeterOntology . 

seas:Multi-jetWaterMeter  a owl:Class ;
                rdfs:comment """Multi-jet meters are very accurate in small sizes and are commonly used for residential and small commercial users. 
                           Multi-jet meters use multiple ports surrounding an internal chamber to create multiple jets of water against an impeller, 
                           whose rotation speed depends on the velocity of water flow. Multi-jets are very accurate at low flow rates, 
                           but there are no large size meters since they do not have the straight-through flow path needed for the high flow rates used in large pipe diameters."""^^xsd:string ;
                rdfs:label "Multi-jet Water Meter"^^xsd:string ;
                rdfs:subClassOf seas:VelocityWaterMeter ;
                vs:term_status "testing"^^xsd:string ;
                rdfs:isDefinedBy seas:SmartMeterOntology .

seas:TurbineWaterMeter  a owl:Class ;
                rdfs:comment """Turbine water meters are less accurate than displacement and jet meters at low flow rates, 
                              but the measuring element does not occupy or severely restrict the entire path of flow. 
                              The flow direction is generally straight through the meter, allowing for higher flow rates and 
                              less pressure loss than displacement-type meters. They are the meter of choice for large 
                              commercial users, fire protection and as master meters for the water distribution system."""^^xsd:string ;
                rdfs:label "Turbine Water Meter"^^xsd:string ;
                rdfs:subClassOf seas:VelocityWaterMeter ;
                vs:term_status "testing"^^xsd:string ;
                rdfs:isDefinedBy seas:SmartMeterOntology .

seas:CompoundWaterMeter  a owl:Class ;
                rdfs:comment """A compound water meter is used where high flow rates are necessary, but where at times there are also smaller rates of 
                                flow that need to be accurately measured. Compound meters have two measuring elements and a check valve 
                                to regulate flow between them. At high flow rates, water is normally diverted primarily or completely 
                                to the high flow element. The high flow element is typically a turbine meter. When flow rates drop to where
                                the high flow element cannot measure accurately, a check valve closes to divert water to a smaller element 
                                that can measure the lower flow rates accurately. The low flow element is typically a multi-jet or PD meter. 
                                By adding the values registered by the high and low elements, the utility has a record of the total consumption 
                                of water flowing through the meter."""^^xsd:string ;
                rdfs:label "Compound Water Meter"^^xsd:string ;
                rdfs:subClassOf seas:VelocityWaterMeter ;
                vs:term_status "testing"^^xsd:string ;
                rdfs:isDefinedBy seas:SmartMeterOntology .

seas:ElectromagneticWaterMeter  a owl:Class ;
                rdfs:comment """Magnetic flow water meters, commonly referred to as "mag meters", are technically a velocity-type water meter, 
                                except that they use electromagnetic properties to determine the water flow velocity, rather than the mechanical 
                                means used by jet and turbine meters. Mag meters use the physics principle of Faraday's law of induction for 
                                measurement, and require AC or DC electricity from a power line or battery to operate the electromagnets. """^^xsd:string ;
                rdfs:label "Electromagnetic Water Meter"^^xsd:string ;
                rdfs:subClassOf seas:WaterMeter ;
                vs:term_status "testing"^^xsd:string ;
                rdfs:isDefinedBy seas:SmartMeterOntology .

seas:UltrasonicWaterMeter  a owl:Class ;
                rdfs:comment """Ultrasonic water meters use one or more ultrasonic transducer to send ultrasonic sound waves 
                                through the fluid to determine the velocity of the water. Since the cross-sectional area of the 
                                meter body is a fixed and known value, when the velocity of water is detected, the volume of 
                                water passing through the meter can be calculated with very high accuracy. Because water density 
                                changes with temperature, most ultrasonic water meters also measure the water temperature as a 
                                component of the volume calculation. """^^xsd:string ;
                rdfs:label "Ultrasonic  Water Meter"^^xsd:string ;
                rdfs:subClassOf seas:WaterMeter ;
                vs:term_status "testing"^^xsd:string ;
                rdfs:isDefinedBy seas:SmartMeterOntology .

seas:GasMeter  a owl:Class ;
                rdfs:comment """A gas meter is a meter, used to measure the volume of fuel gases such as natural gas and propane. 
                            Gas meters are used at residential, commercial, and industrial buildings that consume fuel gas supplied by a gas 
                            utility."""@en;
                rdfs:label "Gas Meter"^^xsd:string ;
                rdfs:subClassOf seas:Meter ;
                rdfs:subClassOf [ owl:onProperty seas:measuresProperty ; owl:someValuesFrom seas:GasVolumeProperty ] ;
                rdfs:subClassOf [ owl:onProperty seas:hasMeteringMechanism ; owl:maxQualifiedCardinality "1"^^xsd:nonNegativeInteger; owl:hasValue seas:MeteringMechanism] ;
                vs:term_status "testing"^^xsd:string ;
                rdfs:isDefinedBy seas:SmartMeterOntology . 

seas:DiaphragmGasMeter  a owl:Class ;
                rdfs:comment """Diaphragm Gas Meter are the most common type of gas meter, seen in almost all residential and small commercial installations.
                                Within the meter there are two or more chambers formed by movable diaphragms. With the gas flow directed by 
                                internal valves, the chambers alternately fill and expel gas, producing a near continuous flow through the meter. 
                                As the diaphragms expand and contract, levers connected to cranks convert the linear motion of the diaphragms into 
                                rotary motion of a crank shaft which serves as the primary flow element. This shaft can drive an odometer-like counter 
                                mechanism or it can produce electrical pulses for a flow computer."""@en;
                rdfs:label "Diaphragm Gas Meter"^^xsd:string ;
                rdfs:subClassOf seas:GasMeter ;
                vs:term_status "testing"^^xsd:string ;
                rdfs:isDefinedBy seas:SmartMeterOntology .

seas:RotaryGasMeter  a owl:Class ;
                rdfs:comment """Rotary gas meters are highly machined precision instruments capable of handling higher volumes 
                                and pressures than diaphragm meters. Within the meter, two figure "8" shaped lobes, the rotors 
                                (also known as impellers or pistons), spin in precise alignment. With each turn, they move a specific quantity 
                                of gas through the meter. The operating principle is similar to that of a Roots blower. The rotational movement 
                                of the crank shaft serves as a primary flow element and may produce electrical pulses for a flow computer or may 
                                drive an odometer-like counter."""@en;
                rdfs:label "Rotary Gas Meter"^^xsd:string ;
                rdfs:subClassOf seas:GasMeter ;
                vs:term_status "testing"^^xsd:string ;
                rdfs:isDefinedBy seas:SmartMeterOntology .

seas:TurbineGasMeter  a owl:Class ;
                rdfs:comment """Turbine gas meters infer gas volume by determining the speed of the gas moving through the meter. 
                                Because the volume of gas is inferred by the flow, it is important that flow conditions are good. 
                                A small internal turbine measures the speed of the gas, which is transmitted mechanically to a mechanical 
                                or electronic counter. These meters do not impede the flow of gas, but are limited at measuring lower flow rates."""@en;
                rdfs:label "Turbine Gas Meter"^^xsd:string ;
                rdfs:subClassOf seas:GasMeter ;
                vs:term_status "testing"^^xsd:string ;
                rdfs:isDefinedBy seas:SmartMeterOntology .

seas:OrificeGasMeter  a owl:Class ;
                rdfs:comment """An orifice gas meter consists of a straight length of pipe inside which a precisely known 
                                orifice creates a pressure drop, thereby affecting flow. Orifice meters are a type of differential meter, 
                                all of which infer the rate of gas flow by measuring the pressure difference across a deliberately designed and 
                                installed flow disturbance. The gas static pressure, density, viscosity, and temperature must be measured or 
                                known in addition to the differential pressure for the meter to accurately measure the fluid. 
                                Orifice meters often do not handle a large range of flow rates. They are however accepted and understood in 
                                industrial applications since they are easy to field-service and have no moving parts."""@en;
                rdfs:label "Orifice Gas Meter"^^xsd:string ;
                rdfs:subClassOf seas:GasMeter ;
                vs:term_status "testing"^^xsd:string ;
                rdfs:isDefinedBy seas:SmartMeterOntology .

seas:UltrasonicFlowGasMeter  a owl:Class ;
                rdfs:comment """Ultrasonic flow gas meters are more complex than meters that are purely mechanical, as they require 
                                significant signal processing and computation capabilities. Ultrasonic meters measure the speed of 
                                gas movement by measuring the speed at which sound travels in the gaseous medium within the pipe. """@en;
                rdfs:label "Ultrasonic flow Gas Meter"^^xsd:string ;
                rdfs:subClassOf seas:GasMeter ;
                vs:term_status "testing"^^xsd:string ;
                rdfs:isDefinedBy seas:SmartMeterOntology .

seas:CoriolisGasMeter  a owl:Class ;
                rdfs:comment """A coriolis meter is usually one or more pipes with longitudinally or axially displaced section(s) 
                                that are excited to vibrate at resonant frequency. Coriolis meters are used with liquids and gases. 
                                When the fluid within the displaced section is at rest, both the upstream and downstream portion of 
                                the displaced section will vibrate in phase with each other. The frequency of this vibration is 
                                determined by the overall density of the pipe (including its contents). This allows the meter to 
                                measure the flowing density of the gas in real time. Once the fluid begins to flow, however, the 
                                coriolis effect comes into play. This effect implies a relationship between the phase difference in 
                                the vibration of the upstream and downstream sections and the mass flow rate of the fluid contained 
                                by the pipe. """@en;
                rdfs:label "Coriolis Gas Meter"^^xsd:string ;
                rdfs:subClassOf seas:GasMeter ;
                vs:term_status "testing"^^xsd:string ;
                rdfs:isDefinedBy seas:SmartMeterOntology .


seas:ElectricityMeter  a owl:Class ;
                rdfs:comment """An electricity meter, electric meter, electrical meter, or energy meter is a meter that measures 
                              the amount of electric energy consumed by a residence, a business, or an electrically powered device."""@en ;
                rdfs:label "Electricity Meter"^^xsd:string ;
                rdfs:subClassOf seas:Meter ;
                rdfs:subClassOf [ owl:onProperty seas:measuresProperty ; owl:someValuesFrom seas:ElectricEnergyProperty ] ;
                rdfs:subClassOf [ owl:onProperty seas:hasMeteringMechanism ; owl:maxQualifiedCardinality "1"^^xsd:nonNegativeInteger; owl:hasValue seas:MeteringMechanism] ;
                vs:term_status "testing"^^xsd:string ;
                rdfs:isDefinedBy seas:SmartMeterOntology . 


seas:ElectromechanicalElectricityMeter  a owl:Class ;
                rdfs:comment """The most common type of electricity meter is the electromechanical induction watt-hour meter.
                                The electromechanical induction meter operates by counting the revolutions of a non-magnetic, 
                                but electrically conductive, metal disc which is made to rotate at a speed proportional to the 
                                power passing through the meter. The number of revolutions is thus proportional to the energy usage. """@en;
                rdfs:label "Electromechanical Electricity Meter"^^xsd:string ;
                rdfs:subClassOf seas:ElectricityMeter ;
                vs:term_status "testing"^^xsd:string ;
                rdfs:isDefinedBy seas:SmartMeterOntology .

seas:ElectronicElectricityMeter  a owl:Class ;
                rdfs:comment """Electronic meters display the energy used on an LCD or LED display, and some can also transmit 
                                readings to remote places. In addition to measuring energy used, electronic meters can also record 
                                other parameters of the load and supply such as instantaneous and maximum rate of usage demands, 
                                voltages, power factor and reactive power used etc. They can also support time-of-day billing, 
                                for example, recording the amount of energy used during on-peak and off-peak hours. """@en;
                rdfs:label "Electronic Electricity Meter"^^xsd:string ;
                rdfs:subClassOf seas:ElectricityMeter ;
                vs:term_status "testing"^^xsd:string ;
                rdfs:isDefinedBy seas:SmartMeterOntology .

seas:SmartMeter a owl:Class;
                rdfs:comment """A smart meter is a meter that records consumption on specific property at regular frequency and 
                                communicates that information at least daily back to the utility for monitoring and billing.
                                A smart meter, is a meter which may be composed of two subSystems : a basic meter to implement a metering 
                                and a connector to read the data and send them to a specific system that can process the data. 
                                The current smartMeter are composition of two systems, but in the future smart meter will be designed to be physicaly a unique system"""@en ;
                rdfs:label "Smart Meter"^^xsd:string ;
                rdfs:subClassOf seas:Meter,                                   
                    [
                      rdf:type owl:Restriction;
                      owl:onProperty seas:hasSubSystem;
                      owl:qualifiedCardinality "1"^^xsd:nonNegativeInteger ;
                      owl:someValuesFrom seas:ConnectorModule
                    ],
                    [
                      rdf:type owl:Restriction;
                      owl:onProperty seas:hasSubSystem;
                      owl:qualifiedCardinality "1"^^xsd:nonNegativeInteger ;
                      owl:someValuesFrom seas:Meter
                    ]
               ;              
               vs:term_status "unstable"^^xsd:string;
               rdfs:isDefinedBy seas:SmartMeterOntology.


seas:WaterSmartMeter a owl:Class;
                    rdfs:label "Water Smart Meter"@en;
                    rdfs:comment """A class of Smart Meter which is used of water metering. Water Smart Meter can only have 
                                  `seas:WaterMeter` as subsystem"""@en;
                    rdfs:subClassOf seas:SmartMeter, 
                    [
                      rdf:type owl:Restriction;
                      owl:onProperty seas:hasSubSystem;
                      owl:qualifiedCardinality "1"^^xsd:nonNegativeInteger ;
                      owl:onClass seas:WaterMeter
                    ];
                    vs:term_status "unstable"^^xsd:string ;
                     rdfs:isDefinedBy seas:SmartMeterOntology.

seas:ElectricitySmartMeter a owl:Class;
                    rdfs:label "Electricity Smart Meter"@en;
                    rdfs:comment """A class of Smart Meter which is used of Electricity metering.
                                    Electricity Smart Meter can only have `seas:ElectricityMeter` as subsystem"""@en;
                    rdfs:subClassOf seas:SmartMeter, 
                    [
                      rdf:type owl:Restriction;
                      owl:onProperty seas:hasSubSystem;
                      owl:qualifiedCardinality "1"^^xsd:nonNegativeInteger ;
                      owl:onClass seas:ElectricityMeter
                    ];
                    vs:term_status "unstable"^^xsd:string ;
                    rdfs:isDefinedBy seas:SmartMeterOntology.


seas:GasSmartMeter a owl:Class;
                    rdfs:label "Gas Smart Meter"@en;
                    rdfs:comment """"A class of Smart Meter which is used of Gas metering.
                                     Gas Smart Meter can only have `seas:GasMeter` as subsystem"""@en;
                    rdfs:subClassOf seas:SmartMeter, 
                    [
                      rdf:type owl:Restriction;
                      owl:onProperty seas:hasSubSystem;
                      owl:qualifiedCardinality "1"^^xsd:nonNegativeInteger ;
                      owl:onClass seas:GasMeter
                    ];
                    vs:term_status "unstable"^^xsd:string ;
                    rdfs:isDefinedBy seas:SmartMeterOntology.

seas:WaterVolumeMetering a owl:Class; 
                        rdfs:subClassOf seas:Metering; 
                        rdfs:comment "The Measure of the volume of the water which flow in the meter"@en;                           
                        rdfs:label "Water Volume Metering"@en;                    
                        vs:term_status "unstable"^^xsd:string  ;
                        rdfs:isDefinedBy seas:SmartMeterOntology . 

seas:WaterVolumeMeteringExecution a owl:Class ;
  rdfs:label "Water Volume Metering Execution"@en ;
  rdfs:comment """A Water Volume Metering Execution is the execution of some Water Volume Metering implemented by some Water Meter."""@en ;
  rdfs:subClassOf seas:MeteringExecution ;
  rdfs:subClassOf [ owl:onProperty pep:executedBy ; owl:someValuesFrom seas:WaterMeter ] ;
  rdfs:subClassOf [ owl:onProperty pep:methodUsed ; owl:someValuesFrom seas:WaterVolumeMetering ] ;
  rdfs:subClassOf [ owl:onProperty seas:measuresProperty ; owl:someValuesFrom seas:WaterVolumeProperty ] ;
  owl:equivalentClass [ owl:onProperty pep:methodUsed ; owl:someValuesFrom seas:WaterVolumeMetering ] ;
  vs:term_status "testing" ;
  rdfs:isDefinedBy seas:SmartMeterOntology . 


seas:GasVolumeMetering a owl:Class; 
                        rdfs:subClassOf seas:Metering; 
                        rdfs:comment "The Measure of the volume of the gas which flow in the meter. Generaly for consumption metering."@en;                           
                        rdfs:label "Gas Volume Metering"@en;                    
                        vs:term_status "unstable"^^xsd:string  ;
                        rdfs:isDefinedBy seas:SmartMeterOntology . 

seas:GasVolumeMeteringExecution a owl:Class ;
  rdfs:label "Gas Volume Metering Execution"@en ;
  rdfs:comment """The Measure of the volume of the gas which flow in the meter. Generaly for consumption metering but could be for production."""@en ;
  rdfs:subClassOf seas:MeteringExecution ;
  rdfs:subClassOf [ owl:onProperty pep:executedBy ; owl:someValuesFrom seas:GasMeter ] ;
  rdfs:subClassOf [ owl:onProperty pep:methodUsed ; owl:someValuesFrom seas:GasVolumeMetering ] ;
  rdfs:subClassOf [ owl:onProperty seas:measuresProperty ; owl:someValuesFrom seas:GasVolumeProperty ] ;
  owl:equivalentClass [ owl:onProperty pep:methodUsed ; owl:someValuesFrom seas:GasVolumeMetering ] ;
  vs:term_status "testing" ;
  rdfs:isDefinedBy seas:SmartMeterOntology . 


seas:ElectricityMetering a owl:Class; 
                        rdfs:subClassOf seas:Metering; 
                        rdfs:comment """The Measure of the electricity which flow through  the meter device.  
                                        It Could be a metering about a consumption or a production of  the electricity"""@en;                           
                        rdfs:label "Electricity Metering"@en;                    
                        vs:term_status "unstable"^^xsd:string  ;
                        rdfs:isDefinedBy seas:SmartMeterOntology . 

seas:ElectricityMeteringExecution a owl:Class ;
  rdfs:label "Electricity Metering Execution"@en ;
  rdfs:comment """An Electricity Metering Execution is the execution of some Electricity Metering process by some electricity meter."""@en ;
  rdfs:subClassOf seas:MeteringExecution ;
  rdfs:subClassOf [ owl:onProperty pep:executedBy ; owl:someValuesFrom seas:ElectricityMeter ] ;
  rdfs:subClassOf [ owl:onProperty pep:methodUsed ; owl:someValuesFrom seas:ElectricityMetering ] ;
  rdfs:subClassOf [ owl:onProperty seas:measuresProperty ; owl:someValuesFrom seas:ElectricEnergyProperty ] ;
  owl:equivalentClass [ owl:onProperty pep:methodUsed ; owl:someValuesFrom seas:ElectricityMetering ] ;
  vs:term_status "testing" ;
  rdfs:isDefinedBy seas:SmartMeterOntology . 



seas:ConsumptionMetering  a owl:Class;
                        rdfs:label "Consumption Metering"@en;
                        rdfs:comment "Any metering about some consumptio. "@en;
                        rdfs:subClassOf  seas:Metering;
                        vs:term_status "testing" ;
                        rdfs:isDefinedBy seas:SmartMeterOntology . 

seas:ProductionMetering  a owl:Class;
                        rdfs:label "Production Metering"@en;
                        rdfs:comment "Any metering about some production."@en;
                        rdfs:subClassOf  seas:Metering;
                        vs:term_status "testing" ;
                        rdfs:isDefinedBy seas:SmartMeterOntology. 


seas:ConsumptionMeteringExecution a owl:Class ;
  rdfs:label "Consumption Metering Execution"@en ;
  rdfs:comment """A Consumption Metering Execution is the execution of some Consumption metering implemented by some meter."""@en ;
  rdfs:subClassOf seas:MeteringExecution ;
  rdfs:subClassOf [ owl:onProperty pep:executedBy ; owl:someValuesFrom seas:Meter ] ;
  rdfs:subClassOf [ owl:onProperty pep:methodUsed ; owl:someValuesFrom seas:ConsumptionMetering ] ;
  rdfs:subClassOf [ owl:onProperty seas:measuresProperty ; owl:someValuesFrom seas:ConsumptionProperty ] ;
  owl:equivalentClass [ owl:onProperty pep:methodUsed ; owl:someValuesFrom seas:ConsumptionMetering ] ;
  vs:term_status "testing" ;
  rdfs:isDefinedBy seas:SmartMeterOntology . 


     
seas:ProductionMeteringExecution a owl:Class ;
  rdfs:label "Production Metering Execution"@en ;
  rdfs:comment """A Productio Metering Execution is the execution of some Production Metering implemented by some meter."""@en ;
  rdfs:subClassOf seas:MeteringExecution ;
  rdfs:subClassOf [ owl:onProperty pep:executedBy ; owl:someValuesFrom seas:Meter ] ;
  rdfs:subClassOf [ owl:onProperty pep:methodUsed ; owl:someValuesFrom seas:ProductionMetering ] ;
  rdfs:subClassOf [ owl:onProperty seas:measuresProperty ; owl:someValuesFrom seas:ProductionProperty ] ;
  owl:equivalentClass [ owl:onProperty pep:methodUsed ; owl:someValuesFrom seas:ProductionMetering ] ;
  vs:term_status "testing" ;
  rdfs:isDefinedBy seas:SmartMeterOntology .                         

###############
# connector module, partie spécifique au connecteur fludia. Est ce qu'il faut la mettre dans une nouvelle onntologie sur les connecteurs fludia ?
# remarque: je ne sais pas trop dans quelle ontology il faut représenter les individus lorsqu'on nous avons besoin ?
###############

seas:FludiaConnectorModule a owl:Class; # the part which is connected to a meter to send the consumption data 
                owl:equivalentClass [ owl:intersectionOf ( seas:ConnectorModule
                                                            [ rdf:type owl:Restriction ;
                                                              owl:onProperty gr:hasManufaturer ;
                                                              owl:hasValue seas:Fludia
                                                            ]
                                                          ) ;
                                     rdf:type owl:Class
                                   ] ;
                rdfs:subClassOf seas:ConnectorModule,
                [owl:onProperty gr:hasManufaturer ; owl:hasValue seas:Fludia];   
                rdfs:label "Fludia Connector Module"@en;
                rdfs:comment "Fludia Connector Module is connector module which is manufactured by fludia."@en;

                vs:term_status "unstable"^^xsd:string ;
                rdfs:isDefinedBy seas:SmartMeterOntology .                         


seas:BelSensoFM420   a owl:Class; # the part which is connected to a meter to send the consumption data 
                    rdfs:label "BelSenso FM420"@en;
                    rdfs:comment "A class of fludia connector which has as model the value `seas:BelSensoFM420Model`"@en;
                   rdfs:subClassOf seas:FludiaConnectorModule,
                  [   owl:onProperty gr:hasMakeAndModel;
                      owl:qualifiedCardinality "1"^^xsd:nonNegativeInteger ;
                      owl:hasValue seas:BelSensoFM420Model
                  ];
                  owl:equivalentClass [ owl:onProperty gr:hasMakeAndModel ; owl:qualifiedCardinality "1"^^xsd:nonNegativeInteger; owl:hasValue seas:BelSensoFM420Model ] ;
                  vs:term_status "unstable"^^xsd:string ;
                 rdfs:isDefinedBy seas:SmartMeterOntology . 

seas:FludiaSigFox a owl:Class;
                       rdfs:label "Fludia Sig Fox"@en;
                       rdfs:comment "A class of fludia connector which communicates with `seas:SigFoxProtocol`."@en;
                      rdfs:subClassOf seas:FludiaConnectorModule,
                      [
                        rdf:type owl:Restriction;
                        owl:onProperty seas:communicatesWithProtocol;
                        owl:qualifiedCardinality "1"^^xsd:nonNegativeInteger ;
                        owl:hasValue seas:SigFoxProtocol
                      ];
                      owl:equivalentClass [ owl:intersectionOf ( seas:FludiaConnectorModule
                                                            [ rdf:type owl:Restriction ;
                                                              owl:onProperty seas:communicatesWithProtocol ;
                                                              owl:hasValue seas:SigFoxProtocol
                                                            ]
                                                          ) ;
                                     rdf:type owl:Class
                                   ] ;
                  
                      vs:term_status "unstable"^^xsd:string ;
                      rdfs:isDefinedBy seas:SmartMeterOntology .                   


seas:FludiaLora a owl:Class;
                       rdfs:label "Fludia Lora"@en;
                       rdfs:comment "A class of fludia connector which communicates with `seas:LoraProtocol`."@en;
                      rdfs:subClassOf seas:FludiaConnectorModule,
                      [
                        rdf:type owl:Restriction;
                        owl:onProperty seas:communicatesWithProtocol;
                        owl:qualifiedCardinality "1"^^xsd:nonNegativeInteger ;
                        owl:hasValue seas:LoraProtocol
                      ];
                      owl:equivalentClass [ owl:intersectionOf ( seas:FludiaConnectorModule
                                                            [ rdf:type owl:Restriction ;
                                                              owl:onProperty seas:communicatesWithProtocol ;
                                                              owl:hasValue seas:LoraProtocol
                                                            ]
                                                          ) ;
                                     rdf:type owl:Class
                                   ] ;
                      vs:term_status "unstable"^^xsd:string ;
                      rdfs:isDefinedBy seas:SmartMeterOntology . 

seas:FludiaModel a owl:Class;                  
                  rdfs:subClassOf gr:ProductOrServiceModel;
                  rdfs:label "Fludia Model"@en;
                  rdfs:comment "The class of model of Fludia such as BelSenso FM 420 Model"@en;
                  vs:term_status "unstable"^^xsd:string ;
                  rdfs:isDefinedBy seas:SmartMeterOntology .

seas:Protocol a owl:Class;
            rdfs:label "Protocol"@en;
            rdfs:comment "A class of protocol which define a set of procedure or rules."@en;
            rdfs:subClassOf seas:System;
            vs:term_status "unstable"^^xsd:string ;
            rdfs:isDefinedBy seas:SmartMeterOntology .

seas:CommunicationsProtocol a owl:Class;
                            rdfs:subClassOf seas:Protocol;
                            rdfs:label "Communications Protocol"@en;
                            rdfs:comment """In telecommunications, a communication protocol is a system of rules that allow two or more entities of a communications system to transmit 
                                          information via any kind of variation of a physical quantity. These are the rules or standard that defines the syntax, semantics and synchronization 
                                          of communication and possible error recovery methods. Protocols may be implemented by hardware, software, or a combination of both"""@en;
                            vs:term_status "unstable"^^xsd:string ;
                            rdfs:isDefinedBy seas:SmartMeterOntology . 

seas:CommunicationsMethod a owl:Class ;
                          rdfs:label "Communications Method"@en;
                          rdfs:comment """Communications methods is a method used to communicate between two Systems. It is a kind of connections. 
                                          Example of methods of communications is `seas:RadioWave`."""@en;
                          rdfs:subClassOf seas:Connection;
                          vs:term_status "unstable"^^xsd:string ;
                          rdfs:isDefinedBy seas:SmartMeterOntology . 

seas:RadioWave a owl:Class;
               rdfs:label "Radio Wave"@en;
               rdfs:comment  """Radio waves are a type of electromagnetic radiation with wavelseasths in the electromagnetic spectrum longer than infrared light. 
                                Radio waves have frequencies from 300 GHz to as low as 3 kHz, and corresponding wavelseasths ranging from 1 millimeter (0.039 in) 4
                                to 100 kilometers (62 mi). Like all other electromagnetic waves, they travel at the speed of light. Naturally occurring radio waves 
                                are made by lightning, or by astronomical objects. Artificially generated radio waves are used for fixed and mobile radio communication, 
                                broadcasting, radar and other navigation systems, communications satellites, computer networks and innumerable other applications. 
                                Radio waves are generated by radio transmitters and received by radio receivers. Different frequencies of radio waves have different 
                                propagati (en)"""@en; 
               rdfs:subClassOf seas:CommunicationsMethod;
               vs:term_status "unstable"^^xsd:string ;
               rdfs:isDefinedBy seas:SmartMeterOntology .

seas:FrequencyProperty a owl:Class; 
                  rdfs:subClassOf seas:Property;
                  rdfs:label "Frequency Property"@en;
                  rdfs:comment "Frequency is the number of occurrences of a repeating event per unit time."@en;
                  vs:term_status "unstable"^^xsd:string;
                  rdfs:isDefinedBy seas:SmartMeterOntology.

seas:FrequencyEvaluation a owl:Class ;
  rdfs:label "Frequency Evaluation"@en;
  rdfs:comment "The class of evaluations for frequency properties."@en ;
  rdfs:subClassOf seas:Evaluation;
  rdfs:subClassOf [ owl:onProperty seas:evaluationOf ; owl:someValuesFrom seas:FrequencyProperty ] ;
  owl:equivalentClass [ owl:onProperty seas:evaluationOf ; owl:allValuesFrom seas:FrequencyProperty ] ;
  vs:term_status "unstable" ;
  rdfs:isDefinedBy seas:SmartMeterOntology.

seas:VolumeProperty a owl:Class;
                        rdfs:subClassOf seas:Property;
                        rdfs:comment """The Volume is a property which is inherent to a physical entity. 
                                      That measure the quantity in three dimensional space. """@en;
                        rdfs:label "Volume Property"@en;
                        vs:term_status "unstable"^^xsd:string;
                        rdfs:isDefinedBy seas:SmartMeterOntology.
                 

seas:VolumeEvaluation a owl:Class ;
  rdfs:label "Volume Evaluation"@en;
  rdfs:comment "The class of evaluations for volume properties."@en ;
  rdfs:subClassOf seas:Evaluation;
  rdfs:subClassOf [ owl:onProperty seas:evaluationOf ; owl:someValuesFrom seas:VolumeProperty ] ;
  owl:equivalentClass [ owl:onProperty seas:evaluationOf ; owl:allValuesFrom seas:VolumeProperty ] ;
  vs:term_status "unstable" ;
  rdfs:isDefinedBy seas:SmartMeterOntology.


seas:WaterVolumeProperty a owl:Class;
                        rdfs:subClassOf seas:VolumeProperty;
                        rdfs:label "Water Volume Property"@en;
                        rdfs:comment "The Water Volume is a property inherent in water. Could be computed in litre or in meter cube. "@en;
                        owl:equivalentClass [ owl:onProperty seas:isPropertyOf ; owl:allValuesFrom seas:Water ] ;
                        vs:term_status "unstable"^^xsd:string;
                        rdfs:isDefinedBy seas:SmartMeterOntology.

seas:WaterVolumeEvaluation a owl:Class ;
  rdfs:label "Water Volume Evaluation"@en;
  rdfs:comment "The class of evaluations for water volume properties."@en ;
  rdfs:subClassOf seas:VolumeEvaluation;
  rdfs:subClassOf [ owl:onProperty seas:evaluationOf ; owl:someValuesFrom seas:WaterVolumeProperty ] ;
  owl:equivalentClass [ owl:onProperty seas:evaluationOf ; owl:allValuesFrom seas:WaterVolumeProperty ] ;
  vs:term_status "unstable" ;
  rdfs:isDefinedBy seas:SmartMeterOntology.

seas:GasVolumeProperty a owl:Class;
                        rdfs:subClassOf seas:VolumeProperty;
                        rdfs:label "Gas Volume Property"@en;
                        rdfs:comment "The Gas Volume is a property inherent in Gas. Could be computed in litre or in meter cube. "@en;
                        owl:equivalentClass [ owl:onProperty seas:isPropertyOf ; owl:allValuesFrom seas:NaturalGas ] ;
                        vs:term_status "unstable"^^xsd:string;
                        rdfs:isDefinedBy seas:SmartMeterOntology.

seas:GasVolumeEvaluation a owl:Class ;
  rdfs:label "Gas Volume Evaluation"@en;
  rdfs:comment "The class of evaluations for Gas volume properties."@en ;
  rdfs:subClassOf seas:VolumeEvaluation;
  rdfs:subClassOf [ owl:onProperty seas:evaluationOf ; owl:someValuesFrom seas:GasVolumeProperty ] ;
  owl:equivalentClass [ owl:onProperty seas:evaluationOf ; owl:allValuesFrom seas:GasVolumeProperty ] ;
  vs:term_status "unstable" ;
  rdfs:isDefinedBy seas:SmartMeterOntology.


seas:ConsumptionProperty a owl:Class;
                        rdfs:subClassOf seas:Property;
                        rdfs:label "Consumption Property"@en;
                        rdfs:comment "The consumption property is a property to measure any consumption."@en;
                        vs:term_status "unstable"^^xsd:string;
                        rdfs:isDefinedBy seas:SmartMeterOntology.

seas:ConsumptionEvaluation a owl:Class ;
  rdfs:label "Consumption Evaluation"@en ;
  rdfs:comment "The class of evaluations for consumption properties."@en ;
  rdfs:subClassOf seas:Evaluation;
  rdfs:subClassOf [ owl:onProperty seas:evaluationOf ; owl:someValuesFrom seas:ConsumptionProperty ] ;
  owl:equivalentClass [ owl:onProperty seas:evaluationOf ; owl:allValuesFrom seas:ConsumptionProperty ] ;
  vs:term_status "unstable" ;
  rdfs:isDefinedBy seas:SmartMeterOntology.

seas:ProductionProperty a owl:Class;
                        rdfs:subClassOf seas:Property;
                        rdfs:label "Production Property"@en;
                        rdfs:comment "The production property is a property to measure any production."@en;
                        vs:term_status "unstable"^^xsd:string;
                        rdfs:isDefinedBy seas:SmartMeterOntology.

seas:ProductionEvaluation a owl:Class ;
  rdfs:label "Production Evaluation"@en ;
  rdfs:comment "The class of evaluations for production properties."@en ;
  rdfs:subClassOf seas:Evaluation;
  rdfs:subClassOf [ owl:onProperty seas:evaluationOf ; owl:someValuesFrom seas:ProductionEvaluation ] ;
  owl:equivalentClass [ owl:onProperty seas:evaluationOf ; owl:allValuesFrom seas:ProductionEvaluation ] ;
  vs:term_status "unstable" ;
  rdfs:isDefinedBy seas:SmartMeterOntology.


seas:AmountOfMatter a owl:Class;
                    rdfs:label "Amount of Matter"@en;
                    rdfs:comment """The common trait of amounts of matter is that they are endurants with no unity 
                                  (according to Gangemi et a. 2001 none of them is an essential  whole). 
                                  Amounts of matter - 'stuffs' referred to by mass nouns like 'gold', 'iron', 'wood',  '
                                  sand', 'meat', etc. - are mereologically  invariant, in the sense that they change their  identity 
                                  when they change some parts."""@en;
                    rdfs:subClassOf seas:FeatureOfInterest;
                    vs:term_status "unstable" ;
                    owl:sameAs <http://www.loa-cnr.it/ontologies/DOLCE-Lite.owl#amount-of-matter>;
                    rdfs:isDefinedBy seas:SmartMeterOntology.

seas:Water a owl:Class;
            rdfs:subClassOf seas:AmountOfMatter;
            rdfs:label "Water"@en ;
            rdfs:comment "Water in its liquid state."@en ;
            vs:term_status "unstable" ;
            rdfs:isDefinedBy seas:SmartMeterOntology.

seas:NaturalGas a owl:Class;
            rdfs:subClassOf seas:AmountOfMatter;
            rdfs:label "Natural Gas"@en ;
            rdfs:comment "Natural Gas in its liquid state."@en ;
            vs:term_status "unstable" ;
            rdfs:isDefinedBy seas:SmartMeterOntology.


######################
# Obejcts and data Properties
###################### 

seas:communicatesWithProtocol rdf:type owl:ObjectProperty;
                              rdfs:label " communicates with protocol"@en;
                              rdfs:comment "Link a system with the communication protocol used to communicate with other systems."@en;
                              rdfs:domain seas:System;
                              rdfs:range  seas:CommunicationsProtocol;
                              vs:term_status "unstable"^^xsd:string ;
                              rdfs:isDefinedBy seas:SmartMeterOntology .

seas:allowsCommunicationsThrough rdf:type owl:ObjectProperty;
                              rdfs:label " allows Communications Through"@en;
                              rdfs:comment "Link a communication protocol with the communication methods used to communicate with other systems."@en;
                              rdfs:domain seas:CommunicationsProtocol;
                              rdfs:range  seas:CommunicationsMethod;
                              vs:term_status "unstable"^^xsd:string ;
                              rdfs:isDefinedBy seas:SmartMeterOntology .


seas:hasSubSystem rdf:type owl:ObjectProperty;
                  rdfs:label "has SubSystem "@en;
                  rdfs:comment "Link a system with its subSystem."@en;
                  owl:inverseOf seas:subSystemOf;
                  rdfs:domain seas:System;
                  rdfs:range seas:System;
                  vs:term_status "unstable"^^xsd:string ;
                  rdfs:isDefinedBy seas:SmartMeterOntology .                               

seas:frequency rdf:type owl:ObjectProperty ; 
                        rdfs:subPropertyOf seas:hasProperty;
                        rdfs:label "frequency"^^xsd:string; 
                        rdfs:domain seas:FeatureOfInterest;                                               
                        rdfs:range seas:FrequencyProperty;
                        rdfs:comment "the frequency relationship connects an entity to the frequency between two successive same kind actions  made by this entity."@en;
                        vs:term_status "unstable"^^xsd:string ;
                        rdfs:isDefinedBy seas:SmartMeterOntology . 

seas:trameSendingFrequency rdf:type owl:ObjectProperty ;    
                        rdfs:subPropertyOf seas:frequency;
                        rdfs:label "trame Sending Frequency"^^xsd:string;  
                         rdfs:domain seas:FeatureOfInterest;                                               
                        rdfs:range seas:FrequencyProperty;                                              
                        rdfs:comment "A trame sending frequency relationship connects an entity to the frequency between two successive sending of trames by the entity"@en;
                        vs:term_status "unstable"^^xsd:string;
                        rdfs:isDefinedBy seas:SmartMeterOntology . 


seas:evaluationFrequency rdf:type owl:ObjectProperty;    
                        rdfs:subPropertyOf seas:frequency;
                        rdfs:label "evaluation frequency"^^xsd:string;                                                
                        rdfs:comment "An evaluation frequency relationship connects an entity to the frequency between two successive evaluations given by the entity"@en;
                        rdfs:domain seas:FeatureOfInterest;                                               
                        rdfs:range seas:FrequencyProperty;
                        vs:term_status "unstable"^^xsd:string  ;
                        rdfs:isDefinedBy seas:SmartMeterOntology .

seas:measuringFrequency rdf:type owl:ObjectProperty ;    
                        rdfs:subPropertyOf seas:frequency;
                        rdfs:label "measuring frequency"^^xsd:string;                                                
                        rdfs:comment "A measuring frequency relationship connects an entity to the frequency between two successives measuring made by the entity"@en;
                        rdfs:domain seas:FeatureOfInterest;                                               
                        rdfs:range seas:FrequencyProperty;
                        vs:term_status "unstable"^^xsd:string  ;
                        rdfs:isDefinedBy seas:SmartMeterOntology .


seas:meteringMechanism rdf:type owl:ObjectProperty ;    
                        rdfs:label "metering mechanism"@en;
                        rdfs:comment "Relation between a Meter and the metering Mechanism or method used for metering. ex: pulse, optic or disc "@en;
                        rdfs:domain seas:Meter;                                                
                        rdfs:range seas:MeteringMechanism ;
                        vs:term_status "unstable"^^xsd:string;
                        rdfs:isDefinedBy seas:SmartMeterOntology .                     



########################
#  data property 
########################

seas:installationIndexValue  rdf:type owl:DatatypeProperty ;
                        rdfs:label "installation index value"^^xsd:string;
                        rdfs:comment "link the smartMeter to the value of the index when the installation. "@en;
                        rdfs:domain seas:SmartMeter;
                        rdfs:range xsd:integer; #  
                        vs:term_status "unstable"^^xsd:string ;
                        rdfs:isDefinedBy seas:SmartMeterOntology .                     

seas:hasInstallationDate  rdf:type owl:DatatypeProperty ;
                        rdfs:label "has installation date"^^xsd:string; # 
                        rdfs:comment "link the smartMeter to the installation installation. "@en;
                        rdfs:domain seas:SmartMeter; 
                        rdfs:range xsd:dateTime;
                        vs:term_status "unstable"^^xsd:string ;
                        rdfs:isDefinedBy seas:SmartMeterOntology .                     

########################
#  some needed instances 
########################

seas:Pulse a seas:MeteringMechanism;
           rdfs:label "Pulse"@en;
           skos:prefLabel "Pulse"@en;
           vs:term_status "unstable"^^xsd:string ;
           rdfs:isDefinedBy seas:SmartMeterOntology .


seas:Disc a seas:MeteringMechanism;
           rdfs:label "Disc"@en;
           skos:prefLabel "Disc"@en;
           vs:term_status "unstable"^^xsd:string ;
           rdfs:isDefinedBy seas:SmartMeterOntology .

seas:Optic a seas:MeteringMechanism;
           rdfs:label "Optic"@en;
           skos:prefLabel "Optic"@en;
           vs:term_status "unstable"^^xsd:string ;
           rdfs:isDefinedBy seas:SmartMeterOntology .

seas:SigFoxProtocol a seas:CommunicationsProtocol;
     rdfs:label "SigFoxProtocol"@en;
     rdfs:comment """The sigFox is defined like this 

```
seas:SigFoxProtocol a seas:CommunicationsProtocol;
                    rdfs:label "SigFoxProtocol"@en;
                    skos:prefLabel "SigFox"@en;
                    gr:hasManufaturer seas:SigFoxCampagny;
                    seas:allowsCommunicationsThrough seas:RadioWave.
```
"""@en ;
     skos:prefLabel "SigFox"@en;
     gr:hasManufaturer seas:SigFoxCampagny;
     seas:allowsCommunicationsThrough seas:radioWave;
     vs:term_status "unstable"^^xsd:string ;
     rdfs:isDefinedBy seas:SmartMeterOntology .

seas:LoraProtocol a seas:CommunicationsProtocol;
      rdfs:label "Lora"@en;
      skos:prefLabel "Lora"@en;
      rdfs:comment """Long Range Wide Area Network, Lora is defined like this 

```
 seas:LoraProtocol  a seas:CommunicationsProtocol;
                    rdfs:label "Lora"@en;
                    skos:prefLabel "Lora"@en;
                    rdfs:comment "Long Range Wide Area Network"@en;
                    owl:sameAs dbr:LoRaWAN. # 
```
"""@en ;
      owl:sameAs dbr:LoRaWAN;
      vs:term_status "unstable"^^xsd:string ;
      rdfs:isDefinedBy seas:SmartMeterOntology .


seas:RadioWave a seas:RadioWave;
    skos:prefLabel "Radio Wave"@en;
    rdfs:label "Radio Wave"@en;
    rdfs:seeAlso dbr:Radio_wave;
    rdfs:comment """The Fludia is defined like this 

```
seas:RadioWaves a seas:RadioWave;
                skos:prefLabel "Radio Wave"@en;
                rdfs:label "Radio Wave"@en;
                rdfs:seeAlso dbr:Radio_wave.
```
"""@en ;
   vs:term_status "unstable"^^xsd:string ;
   rdfs:isDefinedBy seas:SmartMeterOntology .


seas:Fludia a gr:BusinessEntity;
    skos:prefLabel "Fludia"@en;
    rdfs:label "Fludia"@en;
    foaf:homePage <https://www.fludia.com>;
     rdfs:comment """The Fludia is defined like this 

```
seas:Fludia a gr:BusinessEntity;
            skos:prefLabel "Fludia"@en;
            rdfs:label "Fludia"@en;
            foaf:homePage <https://www.fludia.com>.
```
"""@en ;
    vs:term_status "unstable"^^xsd:string ;
    rdfs:isDefinedBy seas:SmartMeterOntology . 


seas:SigFoxCampagny a gr:BusinessEntity;
    rdfs:label "SigFox"@en;
    skos:prefLabel "SigFox"@en;
    foaf:homePage <https://www.sigfox.com>;
    owl:sameAs dbr:Sigfox;
    rdfs:comment """The sigFox compagny is defined like this 

```
seas:SigFoxCampagny a gr:BusinessEntity;
                    rdfs:label "SigFox"@en;
                    skos:prefLabel "SigFox"@en;
                    foaf:homePage <https://www.sigfox.com>;
                    owl:sameAs dbr:Sigfox.
```
"""@en ;
    vs:term_status "unstable"^^xsd:string ;
    rdfs:isDefinedBy seas:SmartMeterOntology .  


seas:BelSensoFM420Model a seas:FludiaModel;
                    rdfs:label "BelSonsoFM20Model"@en;
                    rdfs:comment """BelSonsoFM20 is a model designed by `seas:Fludia`

```
seas:BelSensoFM420Model a seas:FludiaModel;
                        rdfs:label "BelSonsoFM20Model"@en.
```
"""@en ;
                    vs:term_status "unstable"^^xsd:string ;
                    rdfs:isDefinedBy seas:SmartMeterOntology .
